Client04 Adequacy

src/example/Client04.v
@@ -6,11 +6,13 @@ From Fairness Require Import FairBeh Mod Concurrency Linking.
 From Fairness Require Import PCM IProp IPM IPropAux.
 From Fairness Require Import IndexedInvariants OpticsInterp SimWeakest SimWeakestAdequacy.
 From Fairness Require Import TemporalLogic SCMemSpec LifetimeRA AuthExclsRA.
+Require Import Setoid.
 
 Module Client04.
 
   Definition gvs : list nat := [1].
   Definition X := SCMem.val_ptr (0, 0).
+  Global Opaque X.
 
   Section CODE.
 
@@ -34,6 +36,7 @@ Module Client04.
         ITree.iter (fun (_ : unit) =>
                       _ <- (OMod.call (R:=unit) "store" (X, (SCMem.val_nat 1)));;
                       a <- load_loop (SCMem.val_nat 1);;
+                      _ <- trigger Yield;;
                       _ <- (match a with
                             | SCMem.val_nat n => trigger (Observe 0 [n])
                             | _ => UB
@@ -47,6 +50,7 @@ Module Client04.
         ITree.iter (fun (_ : unit) =>
                       _ <- (OMod.call (R:=unit) "store" (X, (SCMem.val_nat 2)));;
                       a <- load_loop (SCMem.val_nat 2);;
+                      _ <- trigger Yield;;
                       _ <- (match a with
                             | SCMem.val_nat n => trigger (Observe 0 [n])
                             | _ => UB
@@ -126,113 +130,67 @@ Section SPEC.
   Lemma mask_disjoint_N_Client04_state_tgt : (↑N_Client04 : coPset) ## (↑N_state_tgt : coPset).
   Proof. apply ndot_ne_disjoint. ss. Qed.
 
-  Definition client04Inv n γi γs1 γs2 γm1 γm2 : sProp (1+n) :=
+  Definition client04Inv n γi γi1 γi2 γs1 γs2 γm1 γm2 : sProp (1+n) :=
     (∃ (tid1 tid2 γ1 γ2 k1 k2 : τ{nat, 1+n}),
       (⤉ ● γs1 (tid1, k1, γ1))
       ∗ (⤉ ● γs2 (tid2, k2, γ2))
       ∗ (⤉ ● γm1 (tid1, k2, γ2))
       ∗ (⤉ ● γm2 (tid2, k1, γ1))
-      ∗ ((⤉ (X ↦ 0))
+      ∗ (((⤉ (X ↦ 0))
           ∗ (⤉ live γi tt 1)
-          ∗ (⤉ Duty (tid1) []) ∗ (⤉ Duty (tid2) [])
+          ∗ (Duty (tid1) []) ∗ (Duty (tid2) [])
           ∗ (⤉ ○ γs1 (tid1, k1, γ1)) ∗ (⤉ ○ γs2 (tid2, k2, γ2)))
         ∨
-        (⤉ dead γi tt)
-          ∗ ((⤉ (X ↦ 1))
-              ∗ (⤉ live γ2 tt 1)
-              ∗ (⤉ (○ γs1 (tid1, k1, γ1)))
-              ∗ (⤉ Duty (tid1) [])
-              ∗ ((⤉ Duty (tid2) [(k2, 1, dead γ2 tt)])
-                  ∗ (◇[k2](2, 1))
-                  ∗ (⤉ (○ γs2 (tid2, k2, γ2))))
-                ∨ (⤉ (○ γm2 (tid2, k1, γ1))))
-            ∨
-            ((⤉ (X ↦ 2))
-              ∗ (⤉ live γ1 tt 1)
-              ∗ (⤉ ○ γs2 (tid2, k2, γ2))
-              ∗ (⤉ Duty (tid2) [])
-              ∗ ((⤉ Duty (tid1) [(k1, 1, dead γ1 tt)])
-                  ∗ (◇[k1](2, 1))
-                  ∗ (⤉ ○ γs1 (tid1, k1, γ1)))
-                ∨ (⤉ (○ γm1 (tid1, k2, γ2)))))%S.
+        ((⤉ dead γi tt)
+          ∗
+          ((⤉ (X ↦ 1))
+            ∗ (⤉ dead γi1 tt)
+            ∗ (⤉ live γ2 tt 1)
+            ∗ (⤉ (○ γs1 (tid1, k1, γ1)))
+            ∗ (Duty (tid1) []) 
+            ∗ (((Duty (tid2) [(k2, 0, dead γ2 tt : sProp (1+n))])
+                ∗ (◇[k2](2, 1))
+                ∗ (⤉ (○ γs2 (tid2, k2, γ2))))
+              ∨ (⤉ (○ γm2 (tid2, k1, γ1))))
+          ∨
+          ((⤉ (X ↦ 2))
+            ∗ (⤉ dead γi2 tt)
+            ∗ (⤉ live γ1 tt 1)
+            ∗ (⤉ ○ γs2 (tid2, k2, γ2))
+            ∗ (Duty (tid2) [])
+            ∗ (((Duty (tid1) [(k1, 0, dead γ1 tt : sProp (1+n))])
+                ∗ (◇[k1](2, 1))
+                ∗ (⤉ ○ γs1 (tid1, k1, γ1)))
+              ∨ (⤉ (○ γm1 (tid1, k2, γ2)))))))))%S.
 
   (** Simulation proof. *)
-  (* Lemma Client04_load_loop_spec
-        tid1 n
-    :
-    ⊢ ⟦(∀ (γi γs1 γs2 γm1 γm2 k2 γ2 : τ{nat, 2+n}),
-           ((⤉ syn_inv (1+n) N_Client04 (client04Inv n γi γs1 γs2 γm1 γm2))
-              ∗ (⤉ syn_tgt_interp_as n sndl (fun m => (s_memory_black m)))
-              ∗ (⤉⤉ ○ γm1 (tid1, k2, γ2))
-              ∗ (⤉⤉ dead γi tt))
-             -∗
-             syn_wpsim (2+n) tid1 ⊤
-             (fun rs rt => (⤉ (syn_term_cond (1+n) tid1 _ rs rt))%S)
-             false false
-             (trigger Yield;;;
-             ` x : () <-
-             (` x : () + () <- (trigger (Observe 0 [2]);;; Ret (inl ()));;
-              match x with
-              | inl l => tau;; ITree.iter (λ _ : (), trigger Yield;;; trigger (Observe 0 [2]);;; Ret (inl ())) l
-              | inr r0 => Ret r0
-              end);; Ret (Any.upcast x))
-            (trigger Yield;;;
-             (` rv : Any.t <- map_event (OMod.emb_callee omod (SCMem.mod gvs)) (Mod.wrap_fun SCMem.store_fun (Any.upcast (X, 1)));;
-              (tau;; unwrap (Any.downcast rv)));;;
-             ` x0 : () + () <-
-             OMod.close_itree omod (SCMem.mod gvs)
-               (` a : SCMem.val <- load_loop 1;;
-                match a with
-                | SCMem.val_nat n0 => trigger (Observe 0 [n0])
-                | SCMem.val_ptr _ => UB
-                end;;; Ret (inl ()));;
-             ` x1 : () <-
-             OMod.close_itree omod (SCMem.mod gvs)
-               match x0 with
-               | inl l =>
-                   tau;; ITree.iter
-                           (λ _ : (),
-                              OMod.call "store" (X, 1);;;
-                              ` a : SCMem.val <- load_loop 1;;
-                              match a with
-                              | SCMem.val_nat n0 => trigger (Observe 0 [n0])
-                              | SCMem.val_ptr _ => UB
-                              end;;; Ret (inl ())) l
-               | inr r0 => Ret r0
-               end;; OMod.close_itree omod (SCMem.mod gvs) (Ret (Any.upcast x1))))%S, 2+n⟧.
-  Admitted. *)
-
-  Lemma Client04_thread1_spec
-        tid1 n
-    :
-    ⊢ ⟦(∀ (γi γs1 γs2 γm1 γm2 k2 γ2 : τ{nat, 2+n}),
-           ((⤉ syn_inv (1+n) N_Client04 (client04Inv n γi γs1 γs2 γm1 γm2))
-              ∗ (⤉ syn_tgt_interp_as n sndl (fun m => (s_memory_black m)))
-              ∗ (⤉⤉ ○ γm1 (tid1, k2, γ2)))
-             -∗
-             syn_wpsim (2+n) tid1 ⊤
-             (fun rs rt => (⤉ (syn_term_cond (1+n) tid1 _ rs rt))%S)
-             false false
-             (fn2th Client04Spec.module "thread1" (tt ↑))
-             (fn2th Client04.module "thread1" (tt ↑)))%S, 2+n⟧.
+  Lemma Client04_load_loop_spec1
+        tid n
+  :
+  ⊢ ∀ (γi γi1 γi2 γs1 γs2 γm1 γm2 k2 γ2 : τ{nat, 2+n}),
+    [@ tid, 1+n, ⊤ @]
+      ⧼⟦((⤉ syn_inv (1+n) N_Client04 (client04Inv n γi γi1 γi2 γs1 γs2 γm1 γm2))
+        ∗ (⤉ syn_tgt_interp_as n sndl (fun m => s_memory_black m))
+        ∗ (⤉⤉ ○ γm1 (tid, k2, γ2))
+        ∗ (⤉⤉ dead γi ())
+        ∗ (⤉⤉ dead γi1 ())
+        ∗ (◆[k2, 2])
+        ∗ (⤉ -[k2](0)-◇ (dead γ2 () : sProp (1+n))))%S, 2+n⟧⧽
+        (OMod.close_itree omod (SCMem.mod gvs) (load_loop 1))
+        ⧼rv, ⌜rv = 2⌝
+          ∗ ∃ k1 γ1, ⟦((⤉⤉ dead γi2 ())
+            ∗ (⤉ Duty (tid) [(k1, 0, dead γ1 tt : sProp (1+n))])
+            ∗ (◇[k1](1, 2))
+            ∗ (⤉⤉ ○ γs1 (tid, k1, γ1)))%S, 2+n⟧⧽
+  .
   Proof.
-    iIntros. red_tl_all. iIntros (γi). red_tl_all. iIntros (γs1).
-    red_tl_all. iIntros (γs2). red_tl_all. iIntros (γm1).
-    red_tl_all. iIntros (γm2). red_tl_all. iIntros (k2).
-    red_tl_all. iIntros (γ2). red_tl_all. simpl. red_tl.
-    iEval (rewrite red_syn_inv; rewrite red_syn_wpsim; rewrite red_syn_tgt_interp_as).
-
-    iIntros "(#INV & #MEM & MY_W)".
-
-    unfold fn2th. simpl. unfold thread1, Client04Spec.thread1.
-    rred2r. lred2r. rewrite ! unfold_iter_eq. rred2r. lred2r.
-    
-    (* Coinduction *)
-    iStopProof. revert k2.
-    eapply wpsim_coind. auto.
-    ii. iIntros "[#HG1 #CIH] [[#INV #MEM] MY_W]".
-    (* Yield *)
-    iEval (rewrite ! unfold_iter_eq). rred2r.
+    iIntros. iStartTriple. simpl. red_tl_all; simpl. rewrite red_syn_inv; rewrite red_syn_tgt_interp_as.
+    iIntros "(#INV & #MEM & WM1 & #DEADI & #DEADI1 & #OBL2 & #PRM2)". iIntros "POST".
+    (* Induction point *)
+    iRevert "WM1 POST".
+    iMod (tpromise_ind with "[] [-]") as "IH"; cycle 2. done. iSplit; done. iModIntro. iIntros "IH". iModIntro.
+    iIntros "WM1 POST". iEval (unfold load_loop at 1; rewrite -> unfold_iter_eq). rred2r.
+    (* clear tid2 γ1 k1. *)
     iInv "INV" as "CI" "CI_CLOSE".
     iEval (unfold client04Inv; red_tl_all; simpl; red_tl) in "CI".
     iDestruct "CI" as "[%tid1' CI]". iEval (red_tl) in "CI".
@@ -240,192 +198,1083 @@ Section SPEC.
     iDestruct "CI" as "[%γ1 CI]". iEval (red_tl) in "CI".
     iDestruct "CI" as "[%γ2' CI]". iEval (red_tl) in "CI".
     iDestruct "CI" as "[%k1 CI]". iEval (red_tl) in "CI".
-    iDestruct "CI" as "[%k2 CI]". iEval (red_tl_all; simpl) in "CI".
-    iDestruct "CI" as "[H0 | [H1 | H2]]"; cycle 1.
-    iDestruct "H1" as "(_ & _ & _ & _ & _ & _ & _ &)
-
-    (* Yield *)
-    iPoseProof (pc_drop _ 1 _ _ 3 with "PCk") as "DROP". eauto. iMod "DROP".
-    iPoseProof (pc_split _ _ 1 2 with "DROP") as "[PC1 PC2]".
-    iApply (wpsim_yieldR with "[DUTY PC1]").
-    { eauto. }
-    { iFrame. simpl. iPoseProof (pcs_cons_fold with "[PC1]") as "FOLD". 2: iFrame. simpl. iFrame. }
-    Unshelve. 2: auto.
-    iIntros "DUTY CRD". rred2r. iApply wpsim_tauR. rred2r.
-
-    iPoseProof (pc_split _ _ 1 1 with "PC2") as "[PC1 PC2]".
-    iApply (wpsim_yieldR with "[DUTY PC1]").
-    { eauto. }
-    { iFrame. simpl. iPoseProof (pcs_cons_fold with "[PC1]") as "FOLD". 2: iFrame. simpl. iFrame. }
-    iIntros "DUTY CRD2". rred2r.
-
-    (* Opening invariant *)
-    iInv "INV" as "CI" "CI_CLOSE".
-    iEval (unfold client01Inv; simpl; red_tl_all; simpl; rewrite red_syn_until_tpromise) in "CI".
-    iDestruct "CI" as "[#OBL UPROMISE]".
-
-    iEval (unfold until_thread_promise; red_tl_all; simpl) in "UPROMISE".
-    iDestruct "UPROMISE" as "[#PRM [BF | #AF]]"; simpl.
-    { (* Live *)
-      iEval (red_tl_all; simpl) in "BF". iDestruct "BF" as "[LIVE2 PT]".
-      (* Store *)
-      iApply (SCMem_store_fun_spec _ _ _ n with "[PT MEM] [ - ]"). auto.
-      { pose mask_disjoint_N_Client01_state_tgt. set_solver. }
-      { iFrame. auto. }
-      iIntros (?) "PTS". rred2r. iApply wpsim_tauR. rred2r.
-
-      iMod ((FUpd_alloc _ _ _ n (N_t1_write) ((X ↦ 1) : sProp n)%S) with "[PTS]") as "#TI". auto.
-      { iEval (simpl; red_tl_all; simpl). auto. }
-      iPoseProof (Lifetime.pending_merge with "LIVE LIVE2") as "LIVE".
-      iEval (rewrite Qp.half_half) in "LIVE". iMod (Lifetime.pending_shot with "LIVE") as "#DEAD".
-      iMod (duty_fulfill with "[DEAD DUTY]") as "DUTY".
-      { iSplitL. iFrame. simpl. red_tl_all. auto. }
-
-      (* Closing the invariant *)
-      iMod ("CI_CLOSE" with "[]") as "_".
-      { iEval (unfold client01Inv; simpl; red_tl_all; simpl).
-        iSplit; [iApply "OBL" | iEval (rewrite red_syn_until_tpromise)].
-        iApply (until_tpromise_make2 with "[]"). simpl. iSplit; auto.
-        iEval (red_tl_all; simpl). iModIntro; iSplit; auto. }
-
-      iApply (wpsim_sync with "[DUTY PC2]").
-      { eauto. }
-      { iFrame. }
-      iIntros "DUTY CRD3". lred2r. rred2r. iApply wpsim_tauR. rred2r.
-      iApply wpsim_ret. eauto. iModIntro.
-      iEval (unfold term_cond). iSplit; iFrame. iPureIntro; auto. }
-    (* After store *)
-    { iEval (unfold t1_write; simpl; red_tl_all; simpl; rewrite red_syn_inv; simpl) in "AF".
-      iDestruct "AF" as "[DEAD _]".
-      iExFalso. iPoseProof (Lifetime.pending_not_shot with "LIVE DEAD") as "%S". auto.
+    iDestruct "CI" as "[%k2' CI]". iEval (red_tl_all; simpl) in "CI".
+    iDestruct "CI" as "(BS1 & BS2 & BM1 & BM2 & [H0 | [_ [H1 | H2]]])".
+    { iDestruct "H0" as "(_ & LIVE & _)". iExFalso; iApply (Lifetime.pending_not_shot with "LIVE"). done. }
+    (* Case 1-1-1 : no one has written when I'm yielding *)
+    { iPoseProof (AuthExcls.b_w_eq with "BM1 WM1") as "%EQ". clarify.
+      iDestruct "H1" as "(PTX & _ & LIVE2 & WS1 & DUTY1 & REST)".
+      (* Yield *)
+      iApply (wpsim_yieldR_gen with "[DUTY1]"). instantiate (1:=1+n). auto. iFrame. iIntros "DUTY1 CRED".
+      iMod ("IH" with "CRED") as "[IH | #DEAD]"; cycle 1.
+      { iExFalso; iApply (Lifetime.pending_not_shot with "LIVE2"). simpl; red_tl_lifetime. done. }
+      iMod ("CI_CLOSE" with "[- WM1 IH POST]") as "_".
+      { iEval (unfold client04Inv; simpl; red_tl).
+        do 6 (iExists _; red_tl); red_tl_all. 
+        iSplitL "BS1"; [done|]. iSplitL "BS2"; [done|]. iSplitL "BM1"; [done|]. iSplitL "BM2"; [done|].
+        iRight. iSplitR; [done | ]. iLeft. simpl. iFrame. done.
+      }
+      iModIntro. rred2r.
+      clear tid2 γ1 k1.
+      iInv "INV" as "CI" "CI_CLOSE".
+      iEval (unfold client04Inv; red_tl_all; simpl; red_tl) in "CI".
+      iDestruct "CI" as "[%tid1' CI]". iEval (red_tl) in "CI".
+      iDestruct "CI" as "[%tid2 CI]". iEval (red_tl) in "CI".
+      iDestruct "CI" as "[%γ1 CI]". iEval (red_tl) in "CI".
+      iDestruct "CI" as "[%γ2' CI]". iEval (red_tl) in "CI".
+      iDestruct "CI" as "[%k1 CI]". iEval (red_tl) in "CI".
+      iDestruct "CI" as "[%k2' CI]". iEval (red_tl_all; simpl) in "CI".
+      iDestruct "CI" as "(BS1 & BS2 & BM1 & BM2 & [H0 | [_ [H1 | H2]]])".
+      { iDestruct "H0" as "(_ & LIVE & _)". iExFalso; iApply (Lifetime.pending_not_shot with "LIVE"). done. }
+      { iPoseProof (AuthExcls.b_w_eq with "BM1 WM1") as "%EQ". clarify.
+        iDestruct "H1" as "(PTX & _ & LIVE_2 & WS1 & DUTY1 & REST)".
+        (* Load 1 - induction by tpromise *)
+        iApply (SCMem_load_fun_spec with "[PTX]"). instantiate (1:=n). auto.
+        { pose mask_disjoint_N_Client04_state_tgt; set_solver. }
+        { iFrame. done. }
+        iIntros (rv') "[% PTX]". subst. rred2r. iApply wpsim_tauR. rred2r.
+        iApply (wpsim_yieldR_gen with "[DUTY1]"). instantiate (1:=1+n). auto. iFrame. iIntros "DUTY1 CRED".
+        iMod ("CI_CLOSE" with "[- WM1 IH POST]") as "_".
+        { iEval (unfold client04Inv; simpl; red_tl).
+          do 6 (iExists _; red_tl); red_tl_all. 
+          iSplitL "BS1"; [done|]. iSplitL "BS2"; [done|]. iSplitL "BM1"; [done|]. iSplitL "BM2"; [done|].
+          iRight. iSplitR; [done | ]. iLeft. simpl. iFrame. done.
+        }
+        iModIntro. rred2r.
+        iApply SCMem_compare_fun_spec. instantiate (1:=n). auto. set_solver.
+        { simpl. des_ifs. iApply (tgt_interp_as_equiv with "MEM"). iIntros. iSplit.
+          { iIntros. simpl. red_tl; simpl. iSplit; [done | iPureIntro; auto]. }
+          { simpl. red_tl; simpl. iIntros "[? _]". done. }
+        }
+        iIntros (rv) "[%EQ _]". exploit EQ. auto. i; subst. rred2r.
+        iApply wpsim_tauR. rred2r. iApply wpsim_tauR. fold (load_loop 1).
+        iApply wpsim_stutter_mon. instantiate (1:=ps); auto. instantiate (1:=pt); auto.
+        iApply ("IH" with "WM1"). done.
+      }
+      { iPoseProof (AuthExcls.b_w_eq with "BM1 WM1") as "%EQ". clarify.
+        iDestruct "H2" as "(PTX & #DEADI2 & LIVE_1 & WS2 & DUTY2 & [(DUTY1 & PC1 & WS1) | MY_W2])"; cycle 1.
+        { iExFalso; iApply (AuthExcls.w_w_false with "WM1 MY_W2"). }
+        iApply (SCMem_load_fun_spec with "[PTX]"). instantiate (1:=n). auto.
+        { pose mask_disjoint_N_Client04_state_tgt; set_solver. }
+        { iFrame. done. }
+        iIntros (rv') "[% PTX]". subst. rred2r. iApply wpsim_tauR. rred2r.
+        iMod (pc_drop _ 1 _ _ 3 with "PC1") as "PC1". auto.
+        iPoseProof (pc_split _ _ 1 2 with "PC1") as "[PC11 PC1]".
+        iApply (wpsim_yieldR_gen with "[DUTY1 PC11]"). instantiate (1:=1+n). auto. iFrame.
+        { iApply pcs_cons_fold. iFrame. } iIntros "DUTY1 CRED".
+        iMod ("CI_CLOSE" with "[- DUTY1 PC1 WS1 POST CRED]") as "_".
+        { iEval (unfold client04Inv; simpl; red_tl).
+          do 6 (iExists _; red_tl); red_tl_all. 
+          iSplitL "BS1"; [done|]. iSplitL "BS2"; [done|]. iSplitL "BM1"; [done|]. iSplitL "BM2"; [done|].
+          iRight. iSplitR; [done | ]. iRight. simpl. iFrame. done.
+        }
+        iModIntro. rred2r.
+        iApply SCMem_compare_fun_spec. instantiate (1:=n). auto. set_solver.
+        { simpl. des_ifs. iApply (tgt_interp_as_equiv with "MEM"). iIntros. iSplit.
+          { iIntros. simpl. red_tl; simpl. iSplit; [done | iPureIntro; auto]. }
+          { simpl. red_tl; simpl. iIntros "[? _]". done. }
+        }
+        iIntros (rv) "[_ %NEQ]". exploit NEQ. auto. i; subst. rred2r.
+        iApply wpsim_tauR. rred2r.
+        iApply ("POST" with "[-]").
+        { iSplit; auto. iExists k1, γ1. red_tl_all; simpl. iFrame. done. }
+      }
     }
+    (* Case 1-1-2 : thread 2 has written when I'm yielding *)
+    iPoseProof (AuthExcls.b_w_eq with "BM1 WM1") as "%EQ". clarify.
+    iDestruct "H2" as "(PTX & #DEADI2 & LIVE_1 & WS2 & DUTY2 & [(DUTY1 & PC1 & WS1) | MY_W2])"; cycle 1.
+    { iExFalso; iApply (AuthExcls.w_w_false with "WM1 MY_W2"). }
+    (* Load 2 *)
+    iMod (pc_drop _ 1 _ _ 4 with "PC1") as "PC1". auto.
+    iPoseProof (pc_split _ _ 1 3 with "PC1") as "[PC11 PC1]".
+    iApply (wpsim_yieldR_gen with "[DUTY1 PC11]"). instantiate (1:=1+n). auto. iFrame.
+    { iApply pcs_cons_fold. iFrame. } iIntros "DUTY1 CRED".
+    iMod ("CI_CLOSE" with "[- DUTY1 PC1 WS1 POST]") as "_".
+    { iEval (unfold client04Inv; simpl; red_tl).
+      do 6 (iExists _; red_tl); red_tl_all. 
+      iSplitL "BS1"; [done|]. iSplitL "BS2"; [done|]. iSplitL "BM1"; [done|]. iSplitL "BM2"; [done|].
+      iRight. iSplitR; [done | ]. iRight. simpl. iFrame. done.
+    }
+    iModIntro. rred2r.
+    iClear "OBL2 PRM2". clear tid2 γ2 k2.
+    iInv "INV" as "CI" "CI_CLOSE".
+    iEval (unfold client04Inv; red_tl_all; simpl; red_tl) in "CI".
+    iDestruct "CI" as "[%tid1' CI]". iEval (red_tl) in "CI".
+    iDestruct "CI" as "[%tid2 CI]". iEval (red_tl) in "CI".
+    iDestruct "CI" as "[%γ1' CI]". iEval (red_tl) in "CI".
+    iDestruct "CI" as "[%γ2 CI]". iEval (red_tl) in "CI".
+    iDestruct "CI" as "[%k1' CI]". iEval (red_tl) in "CI".
+    iDestruct "CI" as "[%k2 CI]". iEval (red_tl_all; simpl) in "CI".
+    iDestruct "CI" as "(BS1 & BS2 & BM1 & BM2 & [H0 | [_ [H1 | H2]]])".
+    { iDestruct "H0" as "(_ & LIVE & _)". iExFalso; iApply (Lifetime.pending_not_shot with "LIVE"). done. }
+    { iDestruct "H1" as "(PTX & _ & LIVE_2 & WS1_2 & DUTY1_2 & _)".
+      iExFalso; iApply (AuthExcls.w_w_false with "WS1 WS1_2").
+    }
+    iDestruct "H2" as "(PTX & _ & LIVE1 & WS2 & DUTY2 & [(_ & _ & WS1_2) | MY_W2])".
+    { iExFalso; iApply (AuthExcls.w_w_false with "WS1 WS1_2"). }
+    iApply (SCMem_load_fun_spec with "[PTX]"). instantiate (1:=n). auto.
+    { pose mask_disjoint_N_Client04_state_tgt; set_solver. }
+    { iFrame. done. }
+    iIntros (rv') "[% PTX]". subst. rred2r. iApply wpsim_tauR. rred2r.
+    iPoseProof (pc_split _ _ 1 2 with "PC1") as "[PC11 PC1]".
+    iApply (wpsim_yieldR_gen with "[DUTY1 PC11]"). instantiate (1:=1+n). auto. iFrame.
+    { iApply pcs_cons_fold. iFrame. } iIntros "DUTY1 _".
+    iMod ("CI_CLOSE" with "[- DUTY1 PC1 WS1 POST]") as "_".
+    { iEval (unfold client04Inv; simpl; red_tl).
+      do 6 (iExists _; red_tl); red_tl_all. 
+      iSplitL "BS1"; [done|]. iSplitL "BS2"; [done|]. iSplitL "BM1"; [done|]. iSplitL "BM2"; [done|].
+      iRight. iSplitR; [done | ]. iRight. simpl. iFrame. done.
+    }
+    iModIntro. rred2r. lred2r.
+    iApply SCMem_compare_fun_spec. instantiate (1:=n). auto. set_solver.
+    { simpl. des_ifs. iApply (tgt_interp_as_equiv with "MEM"). iIntros. iSplit.
+      { iIntros. simpl. red_tl; simpl. iSplit; [done | iPureIntro; auto]. }
+      { simpl. red_tl; simpl. iIntros "[? _]". done. }
+    }
+    iIntros (rv) "[_ %NEQ]". exploit NEQ. auto. i; subst. rred2r.
+    iApply wpsim_tauR. rred2r.
+    iApply ("POST" with "[-]").
+    { iSplit; auto. iExists k1, γ1. red_tl_all; simpl. iFrame. done. }
+  Unshelve. all: auto.
   Qed.
 
-  Lemma Client01_thread2_spec
-        tid n
+  Lemma Client04_thread1_spec
+        tid1 n
     :
-    ⊢ ⟦(∀ (γk k : τ{nat, 1+n}),
-           ((⤉ syn_inv n N_Client04 (client01Inv γk k n))
-              ∗ (syn_tgt_interp_as n sndl (fun m => (s_memory_black m)))
-              ∗ TID(tid) ∗ (⤉ Duty(tid) []))
+    ⊢ ⟦(∀ (γi γi1 γi2 γs1 γs2 γm1 γm2 k2 γ2 : τ{nat, 2+n}),
+           ((⤉ syn_inv (1+n) N_Client04 (client04Inv n γi γi1 γi2 γs1 γs2 γm1 γm2))
+              ∗ (⤉ syn_tgt_interp_as n sndl (fun m => (s_memory_black m)))
+              ∗ (⤉⤉ ○ γm1 (tid1, k2, γ2))
+              ∗ (⤉⤉ live γi1 tt 1))
              -∗
-             syn_wpsim (S n) tid ⊤
-             (fun rs rt => (⤉(syn_term_cond n tid _ rs rt))%S)
+             syn_wpsim (2+n) tid1 ⊤
+             (fun rs rt => (⤉ (syn_term_cond (1+n) tid1 _ rs rt))%S)
              false false
-             (fn2th Client01Spec.module "thread2" (tt ↑))
-             (fn2th Client01.module "thread2" (tt ↑)))%S, 1+n⟧.
+             (fn2th Client04Spec.module "thread1" (tt ↑))
+             (fn2th Client04.module "thread1" (tt ↑)))%S, 2+n⟧.
   Proof.
-    iIntros. red_tl_all. iIntros (γk). red_tl_all. iIntros (k). red_tl_all. simpl.
+    iIntros. red_tl_all. iIntros (γi). red_tl_all. iIntros (γi1).
+    red_tl_all. iIntros (γi2). red_tl_all. iIntros (γs1).
+    red_tl_all. iIntros (γs2). red_tl_all. iIntros (γm1).
+    red_tl_all. iIntros (γm2). red_tl_all. iIntros (k2).
+    red_tl_all. iIntros (γ2). red_tl_all. simpl. red_tl_all.
     iEval (rewrite red_syn_inv; rewrite red_syn_wpsim; rewrite red_syn_tgt_interp_as).
 
-    iIntros "(#INV & #MEM & THDW & DUTY)".
+    iIntros "(#INV & #MEM & MY_W & LIVEI1)".
 
-    unfold fn2th. simpl. unfold thread2, Client01Spec.thread2.
+    unfold fn2th. simpl. unfold thread1, Client04Spec.thread1.
     rred2r. lred2r.
-
-    (* Take steps until the induction point *)
-    iApply (wpsim_yieldR with "[DUTY]").
-    { eauto. }
-    { iFrame. }
-    iIntros "DUTY CRD". rred2r. iApply wpsim_tauR. rred2r.
-    iEval (rewrite unfold_iter_eq; rred2r).
-    iApply (wpsim_yieldR with "[DUTY]").
-    { eauto. }
-    { iFrame. }
-    iIntros "DUTY CRD2". rred2r.
-
-    (* Induction on until_thread_promise *)
+    
+    (* Yield *)
+    iEval (do 2 rewrite unfold_iter_eq). rred2r. lred2r.
     iInv "INV" as "CI" "CI_CLOSE".
-    iEval (unfold client01Inv; simpl; red_tl_all; simpl; rewrite red_syn_until_tpromise; simpl) in "CI".
-    iDestruct "CI" as "[#LOBL UPRM]".
-    iPoseProof (until_tpromise_get_tpromise with "UPRM") as "#TPRM".
-    iRevert "THDW DUTY CI_CLOSE".
-    iMod (until_tpromise_ind with "[LOBL UPRM] [-]") as "IND"; cycle 2.
-    { iApply "IND". }
-    { iSplit; iFrame; auto. }
-    iSplit.
-    (* Not written *)
-    { iModIntro. iIntros "IH". iModIntro. iIntros "PRE THDW DUTY CI_CLOSE".
-      iEval (simpl; red_tl_all; simpl) in "PRE". iDestruct "PRE" as "[LIVE PT]".
-      iApply (SCMem_load_fun_spec _ _ _ n with "[PT MEM] [-]"). auto.
-      { pose mask_disjoint_N_Client01_state_tgt. set_solver. }
-      { iFrame. auto. }
-      iIntros (rv) "[%EQ PTS]"; subst. rred2r. iApply wpsim_tauR. rred2r.
-      (* Yield *)
-      iMod ("CI_CLOSE" with "[LIVE PTS]") as "_".
-      { iEval (unfold client01Inv; simpl; red_tl_all; simpl; unfold until_thread_promise).
-        iSplit; auto.
-        iEval (rewrite red_syn_until_tpromise; simpl; unfold until_thread_promise; simpl;
-            red_tl_all; simpl). iSplit; auto. iLeft. iFrame. }
-      iApply (wpsim_yieldR with "[DUTY]").
-      { eauto. }
-      { iFrame. }
-      iIntros "DUTY CRD". rred2r.
-      (* Compare *)
-      iApply (SCMem_compare_fun_spec). auto. set_solver. simpl.
-      iApply (tgt_interp_as_equiv with "MEM").
-      { iIntros (a). iStartProof. simpl; red_tl_all; simpl. iSplit.
-        { iIntros "MB"; iSplit; iFrame. iPureIntro; auto. }
-        { iIntros "[MB _]"; iFrame. } }
-      iIntros (rv) "[%EQ1 %EQ2]"; hexploit EQ1; auto; intro; subst.
-      rred2r. iApply wpsim_tauR. rred2r. iApply wpsim_tauR.
-      iEval (rewrite unfold_iter_eq; rred2r).
-      iApply (wpsim_yieldR with "[DUTY]").
-      { eauto. }
-      { iFrame. }
-      iIntros "DUTY CRD2". rred2r.
-      
-      (* Appeal to the inductive hypothesis *)
+    iEval (unfold client04Inv; red_tl_all; simpl; red_tl) in "CI".
+    iDestruct "CI" as "[%tid1' CI]". iEval (red_tl) in "CI".
+    iDestruct "CI" as "[%tid2 CI]". iEval (red_tl) in "CI".
+    iDestruct "CI" as "[%γ1 CI]". iEval (red_tl) in "CI".
+    iDestruct "CI" as "[%γ2' CI]". iEval (red_tl) in "CI".
+    iDestruct "CI" as "[%k1 CI]". iEval (red_tl) in "CI".
+    iDestruct "CI" as "[%k2' CI]". iEval (red_tl_all; simpl) in "CI".
+    iDestruct "CI" as "(BS1 & BS2 & BM1 & BM2 & [H0 | [#DEADI [H1 | H2]]])".
+    2:{ iDestruct "H1" as "(_ & #DEAD & _)". iExFalso; iApply (Lifetime.pending_not_shot with "LIVEI1 DEAD "). }
+    (* Case 1 : initialization *)
+    { iDestruct "H0" as "(PTX & LIVEI & DUTY1 & DUTY2 & WS1 & WS2)".
+      iPoseProof (AuthExcls.b_w_eq with "BM1 MY_W") as "%EQ". clarify.
+      iApply (wpsim_yieldR_gen with "[DUTY1]"). instantiate (1:=1+n). auto. iFrame.
+      iIntros "DUTY1 CRED".
+      iMod ("CI_CLOSE" with "[- MY_W CRED LIVEI1]") as "_".
+      { iEval (unfold client04Inv; simpl; red_tl).
+        do 6 (iExists _; red_tl); red_tl_all.
+        iSplitL "BS1"; [done|]. iSplitL "BS2"; [done|]. iSplitL "BM1"; [done|]. iSplitL "BM2"; [done|].
+        iLeft. iFrame.
+      }
+      iModIntro. rred2r. clear tid2 γ1 k1.
       iInv "INV" as "CI" "CI_CLOSE".
-      iEval (unfold client01Inv; simpl; red_tl_all; rewrite red_syn_until_tpromise; simpl) in "CI".
-      iDestruct "CI" as "[_ UPRM]".
-      iMod ("IH" with "[CRD UPRM] ") as "IH". iFrame.
-      iApply ("IH" with "THDW DUTY CI_CLOSE"); iFrame.
+      iEval (unfold client04Inv; red_tl_all; simpl; red_tl) in "CI".
+      iDestruct "CI" as "[%tid1' CI]". iEval (red_tl) in "CI".
+      iDestruct "CI" as "[%tid2 CI]". iEval (red_tl) in "CI".
+      iDestruct "CI" as "[%γ1 CI]". iEval (red_tl) in "CI".
+      iDestruct "CI" as "[%γ2' CI]". iEval (red_tl) in "CI".
+      iDestruct "CI" as "[%k1 CI]". iEval (red_tl) in "CI".
+      iDestruct "CI" as "[%k2' CI]". iEval (red_tl_all; simpl) in "CI".
+      iDestruct "CI" as "(BS1 & BS2 & BM1 & BM2 & [H0 | [#DEADI [H1 | H2]]])".
+      2:{ iDestruct "H1" as "(_ & #DEAD & _)".
+          iExFalso; iApply (Lifetime.pending_not_shot with "LIVEI1 DEAD ").
+      }
+      (* Case 1-1 : no one has written when I'm storing *)
+      { iDestruct "H0" as "(PTX & LIVEI & DUTY1 & DUTY2 & WS1 & WS2)".
+        iPoseProof (AuthExcls.b_w_eq with "BM1 MY_W") as "%EQ". clarify.
+        iApply (SCMem_store_fun_spec with "[PTX] [-]"). instantiate (1:=n). auto.
+        { pose proof mask_disjoint_N_Client04_state_tgt; set_solver. }
+        { iFrame. done. }
+        iIntros (rv) "PTX". rred2r. iApply wpsim_tauR. rred2r.
+        iMod (Lifetime.pending_shot with "LIVEI") as "#DEADI".
+        iMod (Lifetime.pending_shot with "LIVEI1") as "#DEADI1".
+        iMod (Lifetime.alloc tt) as "[%γ2' LIVE2]".
+        iMod (alloc_obligation 2 2) as "[%obl_2 [#OBL_2 PC_2]]".
+        iPoseProof (pc_split _ _ 1 1 with "[PC_2]") as "[PC_21 PC_22]". done.
+        iMod (pc_drop _ 1 _ _ 1 with "PC_22") as "PC_22"; auto.
+        iMod (duty_add (v:=1+n) with "[DUTY2 PC_22] []") as "DUTY2". iFrame.
+        { instantiate (1 := (dead γ2' tt)%S). iEval (simpl; red_tl_all). iModIntro. iIntros "#D". iModIntro. done. }
+        iPoseProof (duty_tpromise with "[DUTY2]") as "#PRM2". 2: done. simpl; left; auto.
+        iMod (AuthExcls.b_w_update _ _ _ (tid2, obl_2, γ2') with "BS2 WS2") as "[BS2 WS2]".
+        iMod (AuthExcls.b_w_update _ _ _ (tid1, obl_2, γ2') with "BM1 MY_W") as "[BM1 MY_W]".
+        clear γ2 k2. rename γ2' into γ2. rename obl_2 into k2.
+        iMod ("CI_CLOSE" with "[- MY_W]") as "_".
+        { iEval (unfold client04Inv; simpl; red_tl).
+          do 6 (iExists _; red_tl); red_tl_all.
+          iSplitL "BS1"; [done|]. iSplitL "BS2"; [done|]. iSplitL "BM1"; [done|]. iSplitL "BM2"; [done|].
+          iRight. iSplitR; [done | ]. iLeft. simpl. iFrame. iSplitR; [done|]. iLeft. iFrame.
+        }
+        (* Coinduction point *)
+        iApply wpsim_reset. iStopProof.
+        pose (k2, γ2) as p. replace k2 with (p.1) by ss. replace γ2 with (p.2) by ss. generalize p. clear p.
+        eapply wpsim_coind. auto. clear k2 γ2.
+        ii. destruct a as [k2 γ2].
+        iIntros "[#HG1 #CIH] [(#INV & #MEM & #DEADI & #DEADI1 & #OBL_2 & #PRM_2) MY_W]". simpl.
+        iApply (Client04_load_loop_spec1 with "[MY_W] [-]").
+        { simpl. red_tl_all; simpl. rewrite red_syn_inv; rewrite red_syn_tgt_interp_as; red_tl_all.
+          iFrame. do 5 (iSplit; [done | ]). done. }
+        iIntros (rv') "(%EQ & %k0 & %γ0 & POST)"; subst. iEval (simpl; red_tl_all; simpl) in "POST".
+        iDestruct "POST" as "(#DEADI2 & DUTY1 & PC1 & WS1)". rred2r.
+        iPoseProof (pc_split _ _ 1 1 with "PC1") as "[PC11 PC1]".
+        iApply (wpsim_sync_gen with "[DUTY1 PC11]"). instantiate (1:=1+n). auto.
+        { iFrame. iApply pcs_cons_fold; iFrame. }
+        iIntros "DUTY1 _". iModIntro. lred2r. rred2r. iApply wpsim_tauR. rred2r.
+        iApply wpsim_observe. iIntros. rred2r. lred2r.
+        iApply wpsim_tauR. iApply wpsim_tauL. rred2r. lred2r. iApply wpsim_tauR.
+        do 2 rewrite unfold_iter_eq. lred2r. rred2r.
+        iApply (wpsim_yieldR_gen with "[DUTY1 PC1]"). instantiate (1:=1+n). auto. iFrame.
+        { iApply pcs_cons_fold; iFrame. }
+        iIntros "DUTY1 _". iModIntro. rred2r.
+        (* Write 1 *)
+        iClear "OBL_2 PRM_2". clear tid2 γ2 k2.
+        iInv "INV" as "CI" "CI_CLOSE".
+        iEval (unfold client04Inv; red_tl_all; simpl; red_tl) in "CI".
+        iDestruct "CI" as "[%tid1' CI]". iEval (red_tl) in "CI".
+        iDestruct "CI" as "[%tid2 CI]". iEval (red_tl) in "CI".
+        iDestruct "CI" as "[%γ1' CI]". iEval (red_tl) in "CI".
+        iDestruct "CI" as "[%γ2 CI]". iEval (red_tl) in "CI".
+        iDestruct "CI" as "[%k1' CI]". iEval (red_tl) in "CI".
+        iDestruct "CI" as "[%k2 CI]". iEval (red_tl_all; simpl) in "CI".
+        iDestruct "CI" as "(BS1 & BS2 & BM1 & BM2 & [H0 | [_ [H1 | H2]]])".
+        { iDestruct "H0" as "(_ & LIVE & _)". iExFalso; iApply (Lifetime.pending_not_shot with "LIVE"). done. }
+        { iDestruct "H1" as "(PTX & _ & LIVE_2 & WS1_2 & DUTY1_2 & _)".
+          iExFalso; iApply (AuthExcls.w_w_false with "WS1 WS1_2").
+        }
+        iDestruct "H2" as "(PTX & _ & LIVE_1 & WS2 & DUTY2 & [(_ & _ & WS1_2) | MY_W2])".
+        { iExFalso; iApply (AuthExcls.w_w_false with "WS1 WS1_2"). }
+        iPoseProof (AuthExcls.b_w_eq with "BS1 WS1") as "%EQ". clarify.
+        iApply (SCMem_store_fun_spec with "[PTX] [-]"). instantiate (1:=n). auto.
+        { pose proof mask_disjoint_N_Client04_state_tgt; set_solver. }
+        { iFrame. done. }
+        iIntros (rv') "PTX". rred2r. iApply wpsim_tauR. rred2r.
+        iMod (Lifetime.pending_shot with "LIVE_1") as "#DEAD_1".
+        iMod (duty_fulfill (v:=1+n) with "[DUTY1]") as "DUTY1". iFrame. simpl; red_tl_lifetime; done.
+        iMod (Lifetime.alloc tt) as "[%γ2' LIVE2]".
+        iMod (alloc_obligation 2 2) as "[%obl_2 [#OBL_2 PC_2]]".
+        iPoseProof (pc_split _ _ 1 1 with "[PC_2]") as "[PC_21 PC_22]". done.
+        iMod (pc_drop _ 1 _ _ 1 with "PC_22") as "PC_22"; auto.
+        iMod (duty_add (v:=1+n) with "[DUTY2 PC_22] []") as "DUTY2". iFrame.
+        { instantiate (1 := (dead γ2' tt)%S). iEval (simpl; red_tl_all).
+          iModIntro. iIntros "#D". iModIntro. done.
+        }
+        iPoseProof (duty_tpromise with "[DUTY2]") as "#PRM2". 2: done. simpl; left; auto.
+        iMod (AuthExcls.b_w_update _ _ _ (tid2, obl_2, γ2') with "BS2 WS2") as "[BS2 WS2]".
+        iMod (AuthExcls.b_w_update _ _ _ (tid1, obl_2, γ2') with "BM1 MY_W2") as "[BM1 WM1]".
+        clear γ2 k2. rename γ2' into γ2. rename obl_2 into k2.
+        iMod ("CI_CLOSE" with "[- WM1]") as "_".
+        { iEval (unfold client04Inv; simpl; red_tl).
+          do 6 (iExists _; red_tl); red_tl_all. 
+          iSplitL "BS1"; [done|]. iSplitL "BS2"; [done|]. iSplitL "BM1"; [done|]. iSplitL "BM2"; [done|].
+          iRight. iSplitR; [done | ]. iLeft. simpl. iFrame. iSplitR; [done | ]. iLeft. iFrame.
+        }
+        iApply wpsim_reset. iApply wpsim_base. auto.
+        iApply "CIH". instantiate (1:=(k2, γ2)). iSplitR; iFrame. iModIntro; iFrame.
+        iSplit; [done|]. iSplit; [done|]. iSplit; [done|]. iSplit; [done|]. iSplit; done.
+      }
+      { (* Case 1-2 : thread 2 has written when I'm storing *)
+        iDestruct "H2" as "(PTX & #DEADI2 & LIVE_1 & WS2 & DUTY2 & [(DUTY1 & PC1 & WS1) | MY_W2])"; cycle 1.
+        { iExFalso; iApply (AuthExcls.w_w_false with "MY_W MY_W2"). }
+        iPoseProof (AuthExcls.b_w_eq with "BM1 MY_W") as "%EQ". clarify.
+        iApply (SCMem_store_fun_spec with "[PTX] [-]"). instantiate (1:=n). auto.
+        { pose proof mask_disjoint_N_Client04_state_tgt; set_solver. }
+        { iFrame. done. }
+        iIntros (rv) "PTX". rred2r. iApply wpsim_tauR. rred2r.
+        iMod (Lifetime.pending_shot with "LIVE_1") as "#DEAD_1".
+        iMod (Lifetime.pending_shot with "LIVEI1") as "#DEADI1".
+        iMod (duty_fulfill (v:=1+n) with "[DUTY1]") as "DUTY1". iFrame. simpl; red_tl_lifetime; done.
+        iMod (Lifetime.alloc tt) as "[%γ2' LIVE2]".
+        iMod (alloc_obligation 2 2) as "[%obl_2 [#OBL_2 PC_2]]".
+        iPoseProof (pc_split _ _ 1 1 with "[PC_2]") as "[PC_21 PC_22]". done.
+        iMod (pc_drop _ 1 _ _ 1 with "PC_22") as "PC_22"; auto.
+        iMod (duty_add (v:=1+n) with "[DUTY2 PC_22] []") as "DUTY2". iFrame.
+        { instantiate (1 := (dead γ2' tt)%S). iEval (simpl; red_tl_all).
+          iModIntro. iIntros "#D". iModIntro. done.
+        }
+        iPoseProof (duty_tpromise with "[DUTY2]") as "#PRM2". 2: done. simpl; left; auto.
+        iMod (AuthExcls.b_w_update _ _ _ (tid2, obl_2, γ2') with "BS2 WS2") as "[BS2 WS2]".
+        iMod (AuthExcls.b_w_update _ _ _ (tid1, obl_2, γ2') with "BM1 MY_W") as "[BM1 WM1]".
+        iMod ("CI_CLOSE" with "[- WM1]") as "_".
+        { iEval (unfold client04Inv; simpl; red_tl).
+          do 6 (iExists _; red_tl); red_tl_all. 
+          iSplitL "BS1"; [done|]. iSplitL "BS2"; [done|]. iSplitL "BM1"; [done|]. iSplitL "BM2"; [done|].
+          iRight. iSplitR; [done | ]. iLeft. simpl. iFrame. iSplitR; [done | ]. iLeft. iFrame.
+        }
+        (* Coinduction point *)
+        clear γ2 k2. rename γ2' into γ2. rename obl_2 into k2. iClear "DEAD_1".
+        iApply wpsim_reset. iStopProof.
+        pose (k2, γ2) as p. replace k2 with (p.1) by ss. replace γ2 with (p.2) by ss. generalize p. clear p.
+        eapply wpsim_coind. auto. clear k2 γ2.
+        ii. destruct a as [k2 γ2].
+        iIntros "[#HG1 #CIH] [(#INV & #MEM & #DEADI & #OBL_2 & #DEADI1 & #OBL2 & #PRM2) MY_W]". simpl.
+        iApply (Client04_load_loop_spec1 with "[MY_W] [-]").
+        { simpl. red_tl_all; simpl. rewrite red_syn_inv; rewrite red_syn_tgt_interp_as; red_tl_all.
+          iFrame. do 5 (iSplit; [done | ]). done. }
+        iIntros (rv') "(%EQ & %k0 & %γ0 & POST)"; subst. iEval (simpl; red_tl_all; simpl) in "POST".
+        iDestruct "POST" as "(#DEADI2 & DUTY1 & PC1 & WS1)". rred2r.
+        iPoseProof (pc_split _ _ 1 1 with "PC1") as "[PC11 PC1]".
+        iApply (wpsim_sync_gen with "[DUTY1 PC11]"). instantiate (1:=1+n). auto.
+        { iFrame. iApply pcs_cons_fold; iFrame. }
+        iIntros "DUTY1 _". iModIntro. lred2r. rred2r. iApply wpsim_tauR. rred2r.
+        iApply wpsim_observe. iIntros. rred2r. lred2r.
+        iApply wpsim_tauR. iApply wpsim_tauL. rred2r. lred2r. iApply wpsim_tauR.
+        do 2 rewrite unfold_iter_eq. lred2r. rred2r.
+        iApply (wpsim_yieldR_gen with "[DUTY1 PC1]"). instantiate (1:=1+n). auto. iFrame.
+        { iApply pcs_cons_fold; iFrame. }
+        iIntros "DUTY1 _". iModIntro. rred2r.
+        (* Write 1 *)
+        iClear "OBL2 PRM2 OBL_2". clear tid2 γ2 k2.
+        iInv "INV" as "CI" "CI_CLOSE".
+        iEval (unfold client04Inv; red_tl_all; simpl; red_tl) in "CI".
+        iDestruct "CI" as "[%tid1' CI]". iEval (red_tl) in "CI".
+        iDestruct "CI" as "[%tid2 CI]". iEval (red_tl) in "CI".
+        iDestruct "CI" as "[%γ1' CI]". iEval (red_tl) in "CI".
+        iDestruct "CI" as "[%γ2 CI]". iEval (red_tl) in "CI".
+        iDestruct "CI" as "[%k1' CI]". iEval (red_tl) in "CI".
+        iDestruct "CI" as "[%k2 CI]". iEval (red_tl_all; simpl) in "CI".
+        iDestruct "CI" as "(BS1 & BS2 & BM1 & BM2 & [H0 | [_ [H1 | H2]]])".
+        { iDestruct "H0" as "(_ & LIVE & _)". iExFalso; iApply (Lifetime.pending_not_shot with "LIVE"). done. }
+        { iDestruct "H1" as "(PTX & _ & LIVE_2 & WS1_2 & DUTY1_2 & _)".
+          iExFalso; iApply (AuthExcls.w_w_false with "WS1 WS1_2").
+        }
+        iDestruct "H2" as "(PTX & _ & LIVE_1 & WS2 & DUTY2 & [(_ & _ & WS1_2) | MY_W2])".
+        { iExFalso; iApply (AuthExcls.w_w_false with "WS1 WS1_2"). }
+        iPoseProof (AuthExcls.b_w_eq with "BS1 WS1") as "%EQ". clarify.
+        iApply (SCMem_store_fun_spec with "[PTX] [-]"). instantiate (1:=n). auto.
+        { pose proof mask_disjoint_N_Client04_state_tgt; set_solver. }
+        { iFrame. done. }
+        iIntros (rv') "PTX". rred2r. iApply wpsim_tauR. rred2r.
+        iMod (Lifetime.pending_shot with "LIVE_1") as "#DEAD_1".
+        iMod (duty_fulfill (v:=1+n) with "[DUTY1]") as "DUTY1". iFrame. simpl; red_tl_lifetime; done.
+        iMod (Lifetime.alloc tt) as "[%γ2' LIVE2]".
+        iMod (alloc_obligation 2 2) as "[%obl_2 [#OBL_2 PC_2]]".
+        iPoseProof (pc_split _ _ 1 1 with "[PC_2]") as "[PC_21 PC_22]". done.
+        iMod (pc_drop _ 1 _ _ 1 with "PC_22") as "PC_22"; auto.
+        iMod (duty_add (v:=1+n) with "[DUTY2 PC_22] []") as "DUTY2". iFrame.
+        { instantiate (1 := (dead γ2' tt)%S). iEval (simpl; red_tl_all).
+          iModIntro. iIntros "#D". iModIntro. done.
+        }
+        iPoseProof (duty_tpromise with "[DUTY2]") as "#PRM2". 2: done. simpl; left; auto.
+        iMod (AuthExcls.b_w_update _ _ _ (tid2, obl_2, γ2') with "BS2 WS2") as "[BS2 WS2]".
+        iMod (AuthExcls.b_w_update _ _ _ (tid1, obl_2, γ2') with "BM1 MY_W2") as "[BM1 WM1]".
+        clear γ2 k2. rename γ2' into γ2. rename obl_2 into k2.
+        iMod ("CI_CLOSE" with "[- WM1]") as "_".
+        { iEval (unfold client04Inv; simpl; red_tl).
+          do 6 (iExists _; red_tl); red_tl_all. 
+          iSplitL "BS1"; [done|]. iSplitL "BS2"; [done|]. iSplitL "BM1"; [done|]. iSplitL "BM2"; [done|].
+          iRight. iSplitR; [done | ]. iLeft. simpl. iFrame. iSplitR; [done | ]. iLeft. iFrame.
+        }
+        iApply wpsim_reset. iApply wpsim_base. auto.
+        iApply "CIH". instantiate (1:=(k2, γ2)). iSplitR; iFrame. iModIntro; iFrame.
+        iSplit; [done|]. iSplit; [done|]. iSplit; [done|]. iSplit; [done|]. iSplit; [done | ]. iSplit; done.
+      }
     }
-
-    (* Written *)
-    iModIntro. iIntros "#DEAD THDW DUTY CI_CLOSE".
-    iEval (red_tl_all; unfold t1_write; simpl; red_tl_all; simpl; rewrite red_syn_inv) in "DEAD".
-    iDestruct "DEAD" as "[DEAD WRITE]".
-    iInv "WRITE" as "WI" "WI_CLOSE".
-    iEval (simpl; red_tl_all; simpl) in "WI".
-    (* Load *)
-    iApply (SCMem_load_fun_spec _ _ _ n with "[WI MEM] [-]"). auto.
-    { pose mask_disjoint_N_Client01_state_tgt.
-      pose mask_disjoint_t1_write_state_tgt.
-      pose mask_disjoint_client01. set_solver.
+    (* Case 2 : x points to 2 *)
+    { iPoseProof (AuthExcls.b_w_eq with "BM1 MY_W") as "%EQ". clarify.
+      iDestruct "H2" as "(PTX & #DEADI2 & LIVE1 & WM2 & DUTY2 & [(DUTY1 & PC1 & WS1) | WM1])"; cycle 1.
+      { iExFalso; iApply (AuthExcls.w_w_false with "MY_W WM1"). }
+      iMod (pc_drop _ 1 _ _ 3 with "PC1") as "PC1". auto.
+      iPoseProof (pc_split _ _ 1 2 with "PC1") as "[PC11 PC1]".
+      iApply (wpsim_yieldR_gen with "[DUTY1 PC11]"). instantiate (1:=1+n). auto. iFrame.
+      { iApply (pcs_cons_fold). iFrame. }
+      iIntros "DUTY1 CRED".
+      iMod ("CI_CLOSE" with "[- DUTY1 PC1 WS1 LIVEI1]") as "_".
+      { iEval (unfold client04Inv; simpl; red_tl).
+        do 6 (iExists _; red_tl); red_tl_all.
+        iSplitL "BS1"; [done|]. iSplitL "BS2"; [done|]. iSplitL "BM1"; [done|].
+        iSplitL "BM2"; [done|]. iRight. iSplitR; [done | ]. iRight. simpl.
+        iSplitL "PTX"; [done | ]. iSplitR; [done | ]. iSplitL "LIVE1"; [done | ].
+        iSplitL "WM2"; [done | ]. iSplitL "DUTY2"; [done | ]. iRight. done.
+      }
+      iModIntro. rred2r. clear tid2.
+      iInv "INV" as "CI" "CI_CLOSE".
+      iEval (unfold client04Inv; red_tl_all; simpl; red_tl) in "CI".
+      iDestruct "CI" as "[%tid1' CI]". iEval (red_tl) in "CI".
+      iDestruct "CI" as "[%tid2 CI]". iEval (red_tl) in "CI".
+      iDestruct "CI" as "[%γ1' CI]". iEval (red_tl) in "CI".
+      iDestruct "CI" as "[%γ2' CI]". iEval (red_tl) in "CI".
+      iDestruct "CI" as "[%k1' CI]". iEval (red_tl) in "CI".
+      iDestruct "CI" as "[%k2' CI]". iEval (red_tl_all; simpl) in "CI".
+      iDestruct "CI" as "(BS1 & BS2 & BM1 & BM2 & [H0 | [_ [H1 | H2]]])".
+      { iDestruct "H0" as "(_ & LIVE & _)". iExFalso; iApply (Lifetime.pending_not_shot with "LIVE"). done. }
+      { iDestruct "H1" as "(PTX & _ & _ & WS1' & _)".
+        iExFalso; iApply (AuthExcls.w_w_false with "WS1 WS1'").
+      }
+      iDestruct "H2" as "(PTX & _ & LIVE1 & WS2 & DUTY2 & [(_ & _ & WS1') | WM1])".
+      { iExFalso; iApply (AuthExcls.w_w_false with "WS1 WS1'"). }
+      iPoseProof (AuthExcls.b_w_eq with "BS1 WS1") as "%EQ". clarify.
+      iApply (SCMem_store_fun_spec with "[PTX] [-]"). instantiate (1:=n). auto.
+      { pose proof mask_disjoint_N_Client04_state_tgt; set_solver. }
+      { iFrame. done. }
+      iIntros (rv) "PTX". rred2r. iApply wpsim_tauR. rred2r.
+      iMod (Lifetime.pending_shot with "LIVE1") as "#DEAD1".
+      iMod (Lifetime.pending_shot with "LIVEI1") as "#DEADI1".
+      iMod (duty_fulfill (v:=1+n) with "[DUTY1]") as "DUTY1". iFrame. simpl; red_tl_lifetime; done.
+      clear γ2 k2. iMod (Lifetime.alloc tt) as "[%γ2 LIVE2]".
+      iMod (alloc_obligation 2 2) as "[%k2 [#OBL2 PC2]]".
+      iPoseProof (pc_split _ _ 1 1 with "[PC2]") as "[PC21 PC22]". done.
+      iMod (pc_drop _ 1 _ _ 1 with "PC22") as "PC22"; auto.
+      iMod (duty_add (v:=1+n) with "[DUTY2 PC22] []") as "DUTY2". iFrame.
+      { instantiate (1 := (dead γ2 tt)%S). iEval (simpl; red_tl_all).
+        iModIntro. iIntros "#D". iModIntro. done.
+      }
+      iPoseProof (duty_tpromise with "[DUTY2]") as "#PRM2". 2: done. simpl; left; auto.
+      iMod (AuthExcls.b_w_update _ _ _ (tid2, k2, γ2) with "BS2 WS2") as "[BS2 WS2]".
+      iMod (AuthExcls.b_w_update _ _ _ (tid1, k2, γ2) with "BM1 WM1") as "[BM1 WM1]".
+      iMod ("CI_CLOSE" with "[- WM1]") as "_".
+      { iEval (unfold client04Inv; simpl; red_tl).
+        do 6 (iExists _; red_tl); red_tl_all. 
+        iSplitL "BS1"; [done|]. iSplitL "BS2"; [done|].
+        iSplitL "BM1"; [done|]. iSplitL "BM2"; [done|].
+        iRight. iSplitR; [done | ]. iLeft. simpl. iFrame. iSplitR; [done | ]. iLeft. iFrame.
+      }
+      (* Coinduction point *)
+      iClear "DEAD1".
+      iApply wpsim_reset. iStopProof.
+      pose (k2, γ2) as p. replace k2 with (p.1) by ss. replace γ2 with (p.2) by ss. generalize p. clear p.
+      eapply wpsim_coind. auto. clear k2 γ2.
+      ii. destruct a as [k2 γ2].
+      iIntros "[#HG1 #CIH] [(#INV & #MEM & #DEADI & #OBL_2 & #DEADI1 & #OBL2 & #PRM2) WM1]". simpl.
+      iApply (Client04_load_loop_spec1 with "[WM1] [-]").
+      { simpl. red_tl_all; simpl. rewrite red_syn_inv; rewrite red_syn_tgt_interp_as; red_tl_all.
+        iFrame. do 5 (iSplit; [done | ]). done. }
+      iIntros (rv') "(%EQ & %k0 & %γ0 & POST)"; subst. iEval (simpl; red_tl_all; simpl) in "POST".
+      iDestruct "POST" as "(#DEADI2 & DUTY1 & PC1 & WS1)". rred2r.
+      iPoseProof (pc_split _ _ 1 1 with "PC1") as "[PC11 PC1]".
+      iApply (wpsim_sync_gen with "[DUTY1 PC11]"). instantiate (1:=1+n). auto.
+      { iFrame. iApply pcs_cons_fold; iFrame. }
+      iIntros "DUTY1 _". iModIntro. lred2r. rred2r. iApply wpsim_tauR. rred2r.
+      iApply wpsim_observe. iIntros. rred2r. lred2r.
+      iApply wpsim_tauR. iApply wpsim_tauL. rred2r. lred2r. iApply wpsim_tauR.
+      do 2 rewrite unfold_iter_eq. lred2r. rred2r.
+      iApply (wpsim_yieldR_gen with "[DUTY1 PC1]"). instantiate (1:=1+n). auto. iFrame.
+      { iApply pcs_cons_fold; iFrame. }
+      iIntros "DUTY1 _". iModIntro. rred2r.
+      (* Write 1 *)
+      iClear "OBL2 PRM2 OBL_2". clear tid2 γ2 k2 γ2'.
+      iInv "INV" as "CI" "CI_CLOSE".
+      iEval (unfold client04Inv; red_tl_all; simpl; red_tl) in "CI".
+      iDestruct "CI" as "[%tid1' CI]". iEval (red_tl) in "CI".
+      iDestruct "CI" as "[%tid2 CI]". iEval (red_tl) in "CI".
+      iDestruct "CI" as "[%γ1' CI]". iEval (red_tl) in "CI".
+      iDestruct "CI" as "[%γ2 CI]". iEval (red_tl) in "CI".
+      iDestruct "CI" as "[%k1' CI]". iEval (red_tl) in "CI".
+      iDestruct "CI" as "[%k2 CI]". iEval (red_tl_all; simpl) in "CI".
+      iDestruct "CI" as "(BS1 & BS2 & BM1 & BM2 & [H0 | [_ [H1 | H2]]])".
+      { iDestruct "H0" as "(_ & LIVE & _)". iExFalso; iApply (Lifetime.pending_not_shot with "LIVE"). done. }
+      { iDestruct "H1" as "(PTX & _ & LIVE_2 & WS1_2 & DUTY1_2 & _)".
+        iExFalso; iApply (AuthExcls.w_w_false with "WS1 WS1_2").
+      }
+      iDestruct "H2" as "(PTX & _ & LIVE_1 & WS2 & DUTY2 & [(_ & _ & WS1_2) | MY_W2])".
+      { iExFalso; iApply (AuthExcls.w_w_false with "WS1 WS1_2"). }
+      iPoseProof (AuthExcls.b_w_eq with "BS1 WS1") as "%EQ". clarify.
+      iApply (SCMem_store_fun_spec with "[PTX] [-]"). instantiate (1:=n). auto.
+      { pose proof mask_disjoint_N_Client04_state_tgt; set_solver. }
+      { iFrame. done. }
+      iIntros (rv') "PTX". rred2r. iApply wpsim_tauR. rred2r.
+      iMod (Lifetime.pending_shot with "LIVE_1") as "#DEAD_1".
+      iMod (duty_fulfill (v:=1+n) with "[DUTY1]") as "DUTY1". iFrame. simpl; red_tl_lifetime; done.
+      iMod (Lifetime.alloc tt) as "[%γ2' LIVE2]".
+      iMod (alloc_obligation 2 2) as "[%obl_2 [#OBL_2 PC_2]]".
+      iPoseProof (pc_split _ _ 1 1 with "[PC_2]") as "[PC_21 PC_22]". done.
+      iMod (pc_drop _ 1 _ _ 1 with "PC_22") as "PC_22"; auto.
+      iMod (duty_add (v:=1+n) with "[DUTY2 PC_22] []") as "DUTY2". iFrame.
+      { instantiate (1 := (dead γ2' tt)%S). iEval (simpl; red_tl_all).
+        iModIntro. iIntros "#D". iModIntro. done.
+      }
+      iPoseProof (duty_tpromise with "[DUTY2]") as "#PRM2". 2: done. simpl; left; auto.
+      iMod (AuthExcls.b_w_update _ _ _ (tid2, obl_2, γ2') with "BS2 WS2") as "[BS2 WS2]".
+      iMod (AuthExcls.b_w_update _ _ _ (tid1, obl_2, γ2') with "BM1 MY_W2") as "[BM1 WM1]".
+      clear γ2 k2. rename γ2' into γ2. rename obl_2 into k2.
+      iMod ("CI_CLOSE" with "[- WM1]") as "_".
+      { iEval (unfold client04Inv; simpl; red_tl).
+        do 6 (iExists _; red_tl); red_tl_all. 
+        iSplitL "BS1"; [done|]. iSplitL "BS2"; [done|]. iSplitL "BM1"; [done|]. iSplitL "BM2"; [done|].
+        iRight. iSplitR; [done | ]. iLeft. simpl. iFrame. iSplitR; [done | ]. iLeft. iFrame.
+      }
+      iApply wpsim_reset. iApply wpsim_base. auto.
+      iApply "CIH". instantiate (1:=(k2, γ2)). iSplitR; iFrame. iModIntro; iFrame.
+      iSplit; [done|]. iSplit; [done|]. iSplit; [done|]. iSplit; [done|]. iSplit; [done | ]. iSplit; done.
     }
-    { iFrame; auto. }
-    iIntros (rv) "[%EQ PTS]"; subst. rred2r. iApply wpsim_tauR. rred2r.
-    iMod ("WI_CLOSE" with "[PTS]") as "_".
-    { simpl; iEval (red_tl_all; simpl); auto. }
-    iMod ("CI_CLOSE" with "[]") as "_".
-    { iEval (unfold client01Inv; simpl; red_tl_all; simpl; rewrite red_syn_until_tpromise;
-        unfold until_thread_promise; simpl; red_tl_all; simpl).
-      iSplit; iFrame; auto. }
-
-    iApply (wpsim_yieldR with "[DUTY]").
-    { eauto. }
-    { iFrame. }
-    iIntros "DUTY CRD". rred2r.
-    (* Compare *)
-    iApply (SCMem_compare_fun_spec). auto. set_solver.
-    iApply (tgt_interp_as_equiv with "MEM").
-    { iIntros (a). simpl. iSplit; iIntros "H"; unfold t1_write; simpl; red_tl_all; simpl; iFrame.
-      { iPureIntro. auto. } { iDestruct "H" as "[MB _]"; iFrame. } }
-    iIntros (rv) "[_ %EQ2]"; hexploit EQ2; auto; intro; subst. rred2r.
-    iApply wpsim_tauR. rred2r.
-
-    iApply (wpsim_sync with "[DUTY]").
-    { eauto. }
-    { iFrame. }
-    iIntros "DUTY CRD2". rred2r.
-    iApply wpsim_tauR. rred2r. lred2r.
-
-    (* Return *)
-    iApply wpsim_ret. auto. iModIntro. iFrame. iPureIntro; auto.
+    Unshelve. all: auto.
   Qed.
 
+  Lemma Client04_load_loop_spec2
+        tid n
+  :
+  ⊢ ∀ (γi γi1 γi2 γs1 γs2 γm1 γm2 k1 γ1 : τ{nat, 2+n}),
+    [@ tid, 1+n, ⊤ @]
+      ⧼⟦((⤉ syn_inv (1+n) N_Client04 (client04Inv n γi γi1 γi2 γs1 γs2 γm1 γm2))
+        ∗ (⤉ syn_tgt_interp_as n sndl (fun m => s_memory_black m))
+        ∗ (⤉⤉ ○ γm2 (tid, k1, γ1))
+        ∗ (⤉⤉ dead γi ())
+        ∗ (⤉⤉ dead γi2 ())
+        ∗ (◆[k1, 2])
+        ∗ (⤉ -[k1](0)-◇ (dead γ1 () : sProp (1+n))))%S, 2+n⟧⧽
+        (OMod.close_itree omod (SCMem.mod gvs) (load_loop 2))
+        ⧼rv, ⌜rv = 1⌝
+          ∗ ∃ k2 γ2, ⟦((⤉⤉ dead γi1 ())
+            ∗ (⤉ Duty (tid) [(k2, 0, dead γ2 tt : sProp (1+n))])
+            ∗ (◇[k2](1, 2))
+            ∗ (⤉⤉ ○ γs2 (tid, k2, γ2)))%S, 2+n⟧⧽
+  .
+  Proof.
+    iIntros. iStartTriple. simpl. red_tl_all; simpl. rewrite red_syn_inv; rewrite red_syn_tgt_interp_as.
+    iIntros "(#INV & #MEM & WM2 & #DEADI & #DEADI2 & #OBL1 & #PRM1)". iIntros "POST".
+    (* Induction point *)
+    iRevert "WM2 POST".
+    iMod (tpromise_ind with "[] [-]") as "IH"; cycle 2. done. iSplit; done. iModIntro. iIntros "IH". iModIntro.
+    iIntros "WM2 POST". iEval (unfold load_loop at 1; rewrite -> unfold_iter_eq). rred2r.
+    iInv "INV" as "CI" "CI_CLOSE".
+    iEval (unfold client04Inv; red_tl_all; simpl; red_tl) in "CI".
+    iDestruct "CI" as "[%tid1 CI]". iEval (red_tl) in "CI".
+    iDestruct "CI" as "[%tid2 CI]". iEval (red_tl) in "CI".
+    iDestruct "CI" as "[%γ1' CI]". iEval (red_tl) in "CI".
+    iDestruct "CI" as "[%γ2 CI]". iEval (red_tl) in "CI".
+    iDestruct "CI" as "[%k1' CI]". iEval (red_tl) in "CI".
+    iDestruct "CI" as "[%k2 CI]". iEval (red_tl_all; simpl) in "CI".
+    iDestruct "CI" as "(BS1 & BS2 & BM1 & BM2 & [H0 | [_ [H1 | H2]]])".
+    { iDestruct "H0" as "(_ & LIVE & _)". iExFalso; iApply (Lifetime.pending_not_shot with "LIVE"). done. }
+    { (* Case 1 : thread 1 has written when loading *)
+      iPoseProof (AuthExcls.b_w_eq with "BM2 WM2") as "%EQ". clarify.
+      iDestruct "H1" as "(PTX & #DEADI1 & LIVE2 & WS1 & DUTY1 & [(DUTY2 & PC2 & WS2) | WM2'])"; cycle 1.
+      { iExFalso; iApply (AuthExcls.w_w_false with "WM2 WM2'"). }
+      (* Load 2 *)
+      iMod (pc_drop _ 1 _ _ 4 with "PC2") as "PC2". auto.
+      iPoseProof (pc_split _ _ 1 3 with "PC2") as "[PC21 PC2]".
+      iApply (wpsim_yieldR_gen with "[DUTY2 PC21]"). instantiate (1:=1+n). auto. iFrame.
+      { iApply pcs_cons_fold. iFrame. } iIntros "DUTY2 CRED".
+      iMod ("CI_CLOSE" with "[- DUTY2 PC2 WS2 POST]") as "_".
+      { iEval (unfold client04Inv; simpl; red_tl).
+        do 6 (iExists _; red_tl); red_tl_all. 
+        iSplitL "BS1"; [done|]. iSplitL "BS2"; [done|]. iSplitL "BM1"; [done|]. iSplitL "BM2"; [done|].
+        iRight. iSplitR; [done | ]. iLeft. simpl. iFrame. done.
+      }
+      iModIntro. rred2r.
+      iClear "OBL1 PRM1". clear tid1 γ1 k1.
+      iInv "INV" as "CI" "CI_CLOSE".
+      iEval (unfold client04Inv; red_tl_all; simpl; red_tl) in "CI".
+      iDestruct "CI" as "[%tid1 CI]". iEval (red_tl) in "CI".
+      iDestruct "CI" as "[%tid2' CI]". iEval (red_tl) in "CI".
+      iDestruct "CI" as "[%γ1 CI]". iEval (red_tl) in "CI".
+      iDestruct "CI" as "[%γ2' CI]". iEval (red_tl) in "CI".
+      iDestruct "CI" as "[%k1 CI]". iEval (red_tl) in "CI".
+      iDestruct "CI" as "[%k2' CI]". iEval (red_tl_all; simpl) in "CI".
+      iDestruct "CI" as "(BS1 & BS2 & BM1 & BM2 & [H0 | [_ [H1 | H2]]])".
+      { iDestruct "H0" as "(_ & LIVE & _)". iExFalso; iApply (Lifetime.pending_not_shot with "LIVE"). done. }
+      2:{ iDestruct "H2" as "(PTX & _ & _ & WS2' & _)".
+        iExFalso; iApply (AuthExcls.w_w_false with "WS2 WS2'").
+      }
+      iDestruct "H1" as "(PTX & _ & LIVE2 & WS1 & DUTY1 & [(_ & _ & WS2') | WM2])".
+      { iExFalso; iApply (AuthExcls.w_w_false with "WS2 WS2'"). }
+      iApply (SCMem_load_fun_spec with "[PTX]"). instantiate (1:=n). auto.
+      { pose mask_disjoint_N_Client04_state_tgt; set_solver. }
+      { iFrame. done. }
+      iIntros (rv') "[% PTX]". subst. rred2r. iApply wpsim_tauR. rred2r.
+      iPoseProof (pc_split _ _ 1 2 with "PC2") as "[PC21 PC2]".
+      iApply (wpsim_yieldR_gen with "[DUTY2 PC21]"). instantiate (1:=1+n). auto. iFrame.
+      { iApply pcs_cons_fold. iFrame. } iIntros "DUTY2 _".
+      iMod ("CI_CLOSE" with "[- DUTY2 PC2 WS2 POST]") as "_".
+      { iEval (unfold client04Inv; simpl; red_tl).
+        do 6 (iExists _; red_tl); red_tl_all. 
+        iSplitL "BS1"; [done|]. iSplitL "BS2"; [done|]. iSplitL "BM1"; [done|]. iSplitL "BM2"; [done|].
+        iRight. iSplitR; [done | ]. iLeft. simpl. iFrame. done.
+      }
+      iModIntro. rred2r. lred2r.
+      iApply SCMem_compare_fun_spec. instantiate (1:=n). auto. set_solver.
+      { simpl. des_ifs. iApply (tgt_interp_as_equiv with "MEM"). iIntros. iSplit.
+        { iIntros. simpl. red_tl; simpl. iSplit; [done | iPureIntro; auto]. }
+        { simpl. red_tl; simpl. iIntros "[? _]". done. }
+      }
+      iIntros (rv) "[_ %NEQ]". exploit NEQ. auto. i; subst. rred2r.
+      iApply wpsim_tauR. rred2r.
+      iApply ("POST" with "[-]").
+      { iSplit; auto. iExists k2, γ2. red_tl_all; simpl. iFrame. done. }
+    }
+    { (* Case 2 : no one has written when I'm loading *)
+      iPoseProof (AuthExcls.b_w_eq with "BM2 WM2") as "%EQ". clarify.
+      iDestruct "H2" as "(PTX & _ & LIVE1 & WS2 & DUTY2 & REST)".
+      (* Yield *)
+      iApply (wpsim_yieldR_gen with "[DUTY2]"). instantiate (1:=1+n). auto. iFrame. iIntros "DUTY2 CRED".
+      iMod ("IH" with "CRED") as "[IH | #DEAD]"; cycle 1.
+      { iExFalso; iApply (Lifetime.pending_not_shot with "LIVE1"). simpl; red_tl_lifetime. done. }
+      iMod ("CI_CLOSE" with "[- WM2 IH POST]") as "_".
+      { iEval (unfold client04Inv; simpl; red_tl).
+        do 6 (iExists _; red_tl); red_tl_all.
+        iSplitL "BS1"; [done|]. iSplitL "BS2"; [done|]. iSplitL "BM1"; [done|]. iSplitL "BM2"; [done|].
+        iRight. iSplitR; [done | ]. iRight. simpl. iFrame. done.
+      }
+      iModIntro. rred2r.
+      clear tid1 γ2 k2.
+      iInv "INV" as "CI" "CI_CLOSE".
+      iEval (unfold client04Inv; red_tl_all; simpl; red_tl) in "CI".
+      iDestruct "CI" as "[%tid1 CI]". iEval (red_tl) in "CI".
+      iDestruct "CI" as "[%tid2' CI]". iEval (red_tl) in "CI".
+      iDestruct "CI" as "[%γ1' CI]". iEval (red_tl) in "CI".
+      iDestruct "CI" as "[%γ2 CI]". iEval (red_tl) in "CI".
+      iDestruct "CI" as "[%k1' CI]". iEval (red_tl) in "CI".
+      iDestruct "CI" as "[%k2 CI]". iEval (red_tl_all; simpl) in "CI".
+      iDestruct "CI" as "(BS1 & BS2 & BM1 & BM2 & [H0 | [_ [H1 | H2]]])".
+      { iDestruct "H0" as "(_ & LIVE & _)". iExFalso; iApply (Lifetime.pending_not_shot with "LIVE"). done. }
+      { iPoseProof (AuthExcls.b_w_eq with "BM2 WM2") as "%EQ". clarify.
+        iDestruct "H1" as "(PTX & #DEADI1 & LIVE2 & WS1 & DUTY1 & [(DUTY2 & PC2 & WS2) | WM2'])"; cycle 1.
+        { iExFalso; iApply (AuthExcls.w_w_false with "WM2 WM2'"). }
+        iApply (SCMem_load_fun_spec with "[PTX]"). instantiate (1:=n). auto.
+        { pose mask_disjoint_N_Client04_state_tgt; set_solver. }
+        { iFrame. done. }
+        iIntros (rv') "[% PTX]". subst. rred2r. iApply wpsim_tauR. rred2r.
+        iMod (pc_drop _ 1 _ _ 3 with "PC2") as "PC2". auto.
+        iPoseProof (pc_split _ _ 1 2 with "PC2") as "[PC21 PC2]".
+        iApply (wpsim_yieldR_gen with "[DUTY2 PC21]"). instantiate (1:=1+n). auto. iFrame.
+        { iApply pcs_cons_fold. iFrame. } iIntros "DUTY2 CRED".
+        iMod ("CI_CLOSE" with "[- DUTY2 PC2 WS2 POST CRED]") as "_".
+        { iEval (unfold client04Inv; simpl; red_tl).
+          do 6 (iExists _; red_tl); red_tl_all. 
+          iSplitL "BS1"; [done|]. iSplitL "BS2"; [done|]. iSplitL "BM1"; [done|]. iSplitL "BM2"; [done|].
+          iRight. iSplitR; [done | ]. iLeft. simpl. iFrame. done.
+        }
+        iModIntro. rred2r.
+        iApply SCMem_compare_fun_spec. instantiate (1:=n). auto. set_solver.
+        { simpl. des_ifs. iApply (tgt_interp_as_equiv with "MEM"). iIntros. iSplit.
+          { iIntros. simpl. red_tl; simpl. iSplit; [done | iPureIntro; auto]. }
+          { simpl. red_tl; simpl. iIntros "[? _]". done. }
+        }
+        iIntros (rv) "[_ %NEQ]". exploit NEQ. auto. i; subst. rred2r.
+        iApply wpsim_tauR. rred2r.
+        iApply ("POST" with "[-]").
+        { iSplit; auto. iExists k2, γ2. red_tl_all; simpl. iFrame. done. }
+      }
+      { iPoseProof (AuthExcls.b_w_eq with "BM2 WM2") as "%EQ". clarify.
+        iDestruct "H2" as "(PTX & _ & LIVE1 & WS2 & DUTY2 & REST)".
+        (* Load 1 - induction by tpromise *)
+        iApply (SCMem_load_fun_spec with "[PTX]"). instantiate (1:=n). auto.
+        { pose mask_disjoint_N_Client04_state_tgt; set_solver. }
+        { iFrame. done. }
+        iIntros (rv') "[% PTX]". subst. rred2r. iApply wpsim_tauR. rred2r.
+        iApply (wpsim_yieldR_gen with "[DUTY2]"). instantiate (1:=1+n). auto. iFrame. iIntros "DUTY2 CRED".
+        iMod ("CI_CLOSE" with "[- WM2 IH POST]") as "_".
+        { iEval (unfold client04Inv; simpl; red_tl).
+          do 6 (iExists _; red_tl); red_tl_all. 
+          iSplitL "BS1"; [done|]. iSplitL "BS2"; [done|]. iSplitL "BM1"; [done|]. iSplitL "BM2"; [done|].
+          iRight. iSplitR; [done | ]. iRight. simpl. iFrame. done.
+        }
+        iModIntro. rred2r.
+        iApply SCMem_compare_fun_spec. instantiate (1:=n). auto. set_solver.
+        { simpl. des_ifs. iApply (tgt_interp_as_equiv with "MEM"). iIntros. iSplit.
+          { iIntros. simpl. red_tl; simpl. iSplit; [done | iPureIntro; auto]. }
+          { simpl. red_tl; simpl. iIntros "[? _]". done. }
+        }
+        iIntros (rv) "[%EQ _]". exploit EQ. auto. i; subst. rred2r.
+        iApply wpsim_tauR. rred2r. iApply wpsim_tauR. fold (load_loop 1).
+        iApply wpsim_stutter_mon. instantiate (1:=ps); auto. instantiate (1:=pt); auto.
+        iApply ("IH" with "WM2"). done.
+      }
+    }
+  Unshelve. all: auto.
+  Qed.
+
+  Lemma Client04_thread2_spec
+        tid2 n
+    :
+    ⊢ ⟦(∀ (γi γi1 γi2 γs1 γs2 γm1 γm2 k1 γ1 : τ{nat, 2+n}),
+           ((⤉ syn_inv (1+n) N_Client04 (client04Inv n γi γi1 γi2 γs1 γs2 γm1 γm2))
+              ∗ (⤉ syn_tgt_interp_as n sndl (fun m => (s_memory_black m)))
+              ∗ (⤉⤉ ○ γm2 (tid2, k1, γ1))
+              ∗ (⤉⤉ live γi2 tt 1))
+             -∗
+             syn_wpsim (2+n) tid2 ⊤
+             (fun rs rt => (⤉ (syn_term_cond (1+n) tid2 _ rs rt))%S)
+             false false
+             (fn2th Client04Spec.module "thread2" (tt ↑))
+             (fn2th Client04.module "thread2" (tt ↑)))%S, 2+n⟧.
+  Proof.
+    iIntros. red_tl_all. iIntros (γi). red_tl_all. iIntros (γi1).
+    red_tl_all. iIntros (γi2). red_tl_all. iIntros (γs1).
+    red_tl_all. iIntros (γs2). red_tl_all. iIntros (γm1).
+    red_tl_all. iIntros (γm2). red_tl_all. iIntros (k1).
+    red_tl_all. iIntros (γ1). red_tl_all. simpl. red_tl_all.
+    iEval (rewrite red_syn_inv; rewrite red_syn_wpsim; rewrite red_syn_tgt_interp_as).
+
+    iIntros "(#INV & #MEM & WM2 & LIVEI2)".
+
+    unfold fn2th. simpl. unfold thread2, Client04Spec.thread2.
+    rred2r. lred2r.
+    
+    (* Yield *)
+    iEval (do 2 rewrite unfold_iter_eq). rred2r. lred2r.
+    iInv "INV" as "CI" "CI_CLOSE".
+    iEval (unfold client04Inv; red_tl_all; simpl; red_tl) in "CI".
+    iDestruct "CI" as "[%tid1 CI]". iEval (red_tl) in "CI".
+    iDestruct "CI" as "[%tid2' CI]". iEval (red_tl) in "CI".
+    iDestruct "CI" as "[%γ1' CI]". iEval (red_tl) in "CI".
+    iDestruct "CI" as "[%γ2 CI]". iEval (red_tl) in "CI".
+    iDestruct "CI" as "[%k1' CI]". iEval (red_tl) in "CI".
+    iDestruct "CI" as "[%k2 CI]". iEval (red_tl_all; simpl) in "CI".
+    iDestruct "CI" as "(BS1 & BS2 & BM1 & BM2 & [H0 | [#DEADI [H1 | H2]]])".
+    3:{ iDestruct "H2" as "(_ & #DEAD & _)". iExFalso; iApply (Lifetime.pending_not_shot with "LIVEI2 DEAD "). }
+    (* Case 1 : initialization *)
+    { iDestruct "H0" as "(PTX & LIVEI & DUTY1 & DUTY2 & WS1 & WS2)".
+      iPoseProof (AuthExcls.b_w_eq with "BM2 WM2") as "%EQ". clarify.
+      iApply (wpsim_yieldR_gen with "[DUTY2]"). instantiate (1:=1+n). auto. iFrame.
+      iIntros "DUTY2 CRED".
+      iMod ("CI_CLOSE" with "[- WM2 CRED LIVEI2]") as "_".
+      { iEval (unfold client04Inv; simpl; red_tl).
+        do 6 (iExists _; red_tl); red_tl_all.
+        iSplitL "BS1"; [done|]. iSplitL "BS2"; [done|]. iSplitL "BM1"; [done|]. iSplitL "BM2"; [done|].
+        iLeft. iFrame.
+      }
+      iModIntro. rred2r. clear tid1 γ2 k2.
+      iInv "INV" as "CI" "CI_CLOSE".
+      iEval (unfold client04Inv; red_tl_all; simpl; red_tl) in "CI".
+      iDestruct "CI" as "[%tid1 CI]". iEval (red_tl) in "CI".
+      iDestruct "CI" as "[%tid2' CI]". iEval (red_tl) in "CI".
+      iDestruct "CI" as "[%γ1' CI]". iEval (red_tl) in "CI".
+      iDestruct "CI" as "[%γ2 CI]". iEval (red_tl) in "CI".
+      iDestruct "CI" as "[%k1' CI]". iEval (red_tl) in "CI".
+      iDestruct "CI" as "[%k2 CI]". iEval (red_tl_all; simpl) in "CI".
+      iDestruct "CI" as "(BS1 & BS2 & BM1 & BM2 & [H0 | [#DEADI [H1 | H2]]])".
+      3:{ iDestruct "H2" as "(_ & #DEAD & _)".
+          iExFalso; iApply (Lifetime.pending_not_shot with "LIVEI2 DEAD ").
+      }
+      (* Case 1-1 : no one has written when I'm storing *)
+      { iDestruct "H0" as "(PTX & LIVEI & DUTY1 & DUTY2 & WS1 & WS2)".
+        iPoseProof (AuthExcls.b_w_eq with "BM2 WM2") as "%EQ". clarify.
+        iApply (SCMem_store_fun_spec with "[PTX] [-]"). instantiate (1:=n). auto.
+        { pose proof mask_disjoint_N_Client04_state_tgt; set_solver. }
+        { iFrame. done. }
+        iIntros (rv) "PTX". rred2r. iApply wpsim_tauR. rred2r.
+        iMod (Lifetime.pending_shot with "LIVEI") as "#DEADI".
+        iMod (Lifetime.pending_shot with "LIVEI2") as "#DEADI2".
+        iMod (Lifetime.alloc tt) as "[%γ1' LIVE1]".
+        iMod (alloc_obligation 2 2) as "[%obl1 [#OBL1 PC1]]".
+        iPoseProof (pc_split _ _ 1 1 with "[PC1]") as "[PC11 PC12]". done.
+        iMod (pc_drop _ 1 _ _ 1 with "PC12") as "PC12"; auto.
+        iMod (duty_add (v:=1+n) with "[DUTY1 PC12] []") as "DUTY1". iFrame.
+        { instantiate (1 := (dead γ1' tt)%S). iEval (simpl; red_tl_all). iModIntro. iIntros "#D". iModIntro. done. }
+        iPoseProof (duty_tpromise with "[DUTY1]") as "#PRM2". 2: done. simpl; left; auto.
+        iMod (AuthExcls.b_w_update _ _ _ (tid1, obl1, γ1') with "BS1 WS1") as "[BS1 WS1]".
+        iMod (AuthExcls.b_w_update _ _ _ (tid2, obl1, γ1') with "BM2 WM2") as "[BM2 WM2]".
+        clear γ1 k1. rename γ1' into γ1. rename obl1 into k1.
+        iMod ("CI_CLOSE" with "[- WM2]") as "_".
+        { iEval (unfold client04Inv; simpl; red_tl).
+          do 6 (iExists _; red_tl); red_tl_all.
+          iSplitL "BS1"; [done|]. iSplitL "BS2"; [done|]. iSplitL "BM1"; [done|]. iSplitL "BM2"; [done|].
+          iRight. iSplitR; [done | ]. iRight. simpl. iFrame. iSplitR; [done|]. iLeft. iFrame.
+        }
+        (* Coinduction point *)
+        iApply wpsim_reset. iStopProof.
+        pose (k1, γ1) as p. replace k1 with (p.1) by ss. replace γ1 with (p.2) by ss. generalize p. clear p.
+        eapply wpsim_coind. auto. clear k1 γ1.
+        ii. destruct a as [k1 γ1].
+        iIntros "[#HG1 #CIH] [(#INV & #MEM & #DEADI & #DEADI2 & #OBL1 & #PRM1) WM2]". simpl.
+        iApply (Client04_load_loop_spec2 with "[WM2] [-]").
+        { simpl. red_tl_all; simpl. rewrite red_syn_inv; rewrite red_syn_tgt_interp_as; red_tl_all.
+          iFrame. do 5 (iSplit; [done | ]). done. }
+        iIntros (rv') "(%EQ & %k0 & %γ0 & POST)"; subst. iEval (simpl; red_tl_all; simpl) in "POST".
+        iDestruct "POST" as "(#DEADI1 & DUTY2 & PC2 & WS2)". rred2r.
+        iPoseProof (pc_split _ _ 1 1 with "PC2") as "[PC21 PC2]".
+        iApply (wpsim_sync_gen with "[DUTY2 PC21]").
+        { instantiate (1:=1+n). auto. }
+        { iFrame. iApply (pcs_cons_fold). iSplitL; done. }
+        iIntros "DUTY2 CRED". iModIntro. lred2r. rred2r. iApply wpsim_tauR. rred2r.
+        iApply wpsim_observe. iIntros (ret). lred2r; rred2r.
+        iApply wpsim_tauL; iApply wpsim_tauR. lred2r; rred2r. iApply wpsim_tauR.
+        do 2 rewrite unfold_iter_eq. lred2r. rred2r.
+        iApply (wpsim_yieldR_gen with "[DUTY2 PC2]"). instantiate (1:=1+n). auto. iFrame.
+        { iApply pcs_cons_fold; iFrame. }
+        iIntros "DUTY2 _". iModIntro. rred2r.
+         iClear "OBL1 PRM1". clear tid1 γ1 k1.
+        iInv "INV" as "CI" "CI_CLOSE".
+        iEval (unfold client04Inv; red_tl_all; simpl; red_tl) in "CI".
+        iDestruct "CI" as "[%tid1 CI]". iEval (red_tl) in "CI".
+        iDestruct "CI" as "[%tid2' CI]". iEval (red_tl) in "CI".
+        iDestruct "CI" as "[%γ1 CI]". iEval (red_tl) in "CI".
+        iDestruct "CI" as "[%γ2' CI]". iEval (red_tl) in "CI".
+        iDestruct "CI" as "[%k1 CI]". iEval (red_tl) in "CI".
+        iDestruct "CI" as "[%k2' CI]". iEval (red_tl_all; simpl) in "CI".
+        iDestruct "CI" as "(BS1 & BS2 & BM1 & BM2 & [H0 | [_ [H1 | H2]]])".
+        { iDestruct "H0" as "(_ & LIVE & _)". iExFalso; iApply (Lifetime.pending_not_shot with "LIVE"). done. }
+        2:{ iDestruct "H2" as "(PTX & _ & LIVE1 & WS2' & DUTY2' & _)".
+          iExFalso; iApply (AuthExcls.w_w_false with "WS2 WS2'").
+        }
+        iDestruct "H1" as "(PTX & _ & LIVE2 & WS1 & DUTY1 & [(_ & _ & WS2') | WM2])".
+        { iExFalso; iApply (AuthExcls.w_w_false with "WS2 WS2'"). }
+        iPoseProof (AuthExcls.b_w_eq with "BS2 WS2") as "%EQ". clarify.
+        iApply (SCMem_store_fun_spec with "[PTX] [-]"). instantiate (1:=n). auto.
+        { pose proof mask_disjoint_N_Client04_state_tgt; set_solver. }
+        { iFrame. done. }
+        iIntros (rv') "PTX". rred2r. iApply wpsim_tauR. rred2r.
+        iMod (Lifetime.pending_shot with "LIVE2") as "#DEAD2".
+        iMod (duty_fulfill (v:=1+n) with "[DUTY2]") as "DUTY2". iFrame. simpl; red_tl_lifetime; done.
+        iMod (Lifetime.alloc tt) as "[%γ1' LIVE1]".
+        iMod (alloc_obligation 2 2) as "[%obl1 [#OBL1 PC1]]".
+        iPoseProof (pc_split _ _ 1 1 with "[PC1]") as "[PC11 PC12]". done.
+        iMod (pc_drop _ 1 _ _ 1 with "PC11") as "PC11"; auto.
+        iMod (duty_add (v:=1+n) with "[DUTY1 PC11] []") as "DUTY1". iFrame.
+        { instantiate (1 := (dead γ1' tt)%S). iEval (simpl; red_tl_all).
+          iModIntro. iIntros "#D". iModIntro. done.
+        }
+        iPoseProof (duty_tpromise with "[DUTY1]") as "#PRM1". 2: done. simpl; left; auto.
+        iMod (AuthExcls.b_w_update _ _ _ (tid2, obl1, γ1') with "BM2 WM2") as "[BM2 WM2]".
+        iMod (AuthExcls.b_w_update _ _ _ (tid1, obl1, γ1') with "BS1 WS1") as "[BS1 WS1]".
+        clear γ1 k1. rename γ1' into γ1. rename obl1 into k1.
+        iMod ("CI_CLOSE" with "[- WM2]") as "_".
+        { iEval (unfold client04Inv; simpl; red_tl).
+          do 6 (iExists _; red_tl); red_tl_all. 
+          iSplitL "BS1"; [done|]. iSplitL "BS2"; [done|]. iSplitL "BM1"; [done|]. iSplitL "BM2"; [done|].
+          iRight. iSplitR; [done | ]. iRight. simpl. iFrame. iSplitR; [done | ]. iLeft. iFrame.
+        }
+        iApply wpsim_reset. iApply wpsim_base. auto.
+        iApply "CIH". instantiate (1:=(k1, γ1)). iSplitR; iFrame. iModIntro; iFrame.
+        iSplit; [done|]. iSplit; [done|]. iSplit; [done|]. iSplit; [done|]. iSplit; done.
+      }
+      { (* Case 1-2 : thread 1 has written when I'm storing *)
+        iDestruct "H1" as "(PTX & #DEADI1 & LIVE2 & WS1 & DUTY1 & [(DUTY2 & PC2 & WS2) | WM2'])"; cycle 1.
+        { iExFalso; iApply (AuthExcls.w_w_false with "WM2 WM2'"). }
+        iPoseProof (AuthExcls.b_w_eq with "BM2 WM2") as "%EQ". clarify.
+        iApply (SCMem_store_fun_spec with "[PTX] [-]"). instantiate (1:=n). auto.
+        { pose proof mask_disjoint_N_Client04_state_tgt; set_solver. }
+        { iFrame. done. }
+        iIntros (rv) "PTX". rred2r. iApply wpsim_tauR. rred2r.
+        iMod (Lifetime.pending_shot with "LIVE2") as "#DEAD2".
+        iMod (Lifetime.pending_shot with "LIVEI2") as "#DEADI2".
+        iMod (duty_fulfill (v:=1+n) with "[DUTY2]") as "DUTY2". iFrame. simpl; red_tl_lifetime; done.
+        iMod (Lifetime.alloc tt) as "[%γ1' LIVE1]".
+        iMod (alloc_obligation 2 2) as "[%obl1 [#OBL1 PC1]]".
+        iPoseProof (pc_split _ _ 1 1 with "[PC1]") as "[PC11 PC12]". done.
+        iMod (pc_drop _ 1 _ _ 1 with "PC11") as "PC11"; auto.
+        iMod (duty_add (v:=1+n) with "[DUTY1 PC11] []") as "DUTY1". iFrame.
+        { instantiate (1 := (dead γ1' tt)%S). iEval (simpl; red_tl_all).
+          iModIntro. iIntros "#D". iModIntro. done.
+        }
+        iPoseProof (duty_tpromise with "[DUTY1]") as "#PRM1". 2: done. simpl; left; auto.
+        iMod (AuthExcls.b_w_update _ _ _ (tid2, obl1, γ1') with "BM2 WM2") as "[BM2 WM2]".
+        iMod (AuthExcls.b_w_update _ _ _ (tid1, obl1, γ1') with "BS1 WS1") as "[BS1 WS1]".
+        iMod ("CI_CLOSE" with "[- WM2]") as "_".
+        { iEval (unfold client04Inv; simpl; red_tl).
+          do 6 (iExists _; red_tl); red_tl_all.
+          iSplitL "BS1"; [done|]. iSplitL "BS2"; [done|]. iSplitL "BM1"; [done|]. iSplitL "BM2"; [done|].
+          iRight. iSplitR; [done | ]. iRight. simpl. iFrame. iSplitR; [done | ]. iLeft. iFrame.
+        }
+        (* Coinduction point *)
+        clear γ1 k1. rename γ1' into γ1. rename obl1 into k1. iClear "DEAD2".
+        iApply wpsim_reset. iStopProof.
+        pose (k1, γ1) as p. replace k1 with (p.1) by ss. replace γ1 with (p.2) by ss. generalize p. clear p.
+        eapply wpsim_coind. auto. clear k1 γ1.
+        ii. destruct a as [k1 γ1].
+        iIntros "[#HG1 #CIH] [(#INV & #MEM & #DEADI & #DEADI1 & #DEADI2 & #OBL1 & #PRM1) WM2]". simpl.
+        iApply (Client04_load_loop_spec2 with "[WM2] [-]").
+        { simpl. red_tl_all; simpl. rewrite red_syn_inv; rewrite red_syn_tgt_interp_as; red_tl_all.
+          iFrame. do 5 (iSplit; [done | ]). done. }
+        iIntros (rv') "(%EQ & %k0 & %γ0 & POST)"; subst. iEval (simpl; red_tl_all; simpl) in "POST".
+        iDestruct "POST" as "(_ & DUTY2 & PC2 & WS2)". rred2r.
+        iPoseProof (pc_split _ _ 1 1 with "PC2") as "[PC21 PC2]".
+        iApply (wpsim_sync_gen with "[DUTY2 PC21]").
+        { instantiate (1:=1+n). auto. }
+        { iFrame. iApply (pcs_cons_fold). iSplitL; done. }
+        iIntros "DUTY2 CRED". iModIntro. lred2r. rred2r. iApply wpsim_tauR. rred2r.
+        iApply wpsim_observe. iIntros (ret). lred2r; rred2r.
+        iApply wpsim_tauL; iApply wpsim_tauR. lred2r; rred2r. iApply wpsim_tauR.
+        do 2 rewrite unfold_iter_eq. lred2r. rred2r.
+        iApply (wpsim_yieldR_gen with "[DUTY2 PC2]"). instantiate (1:=1+n). auto. iFrame.
+        { iApply pcs_cons_fold; iFrame. }
+        iIntros "DUTY2 _". iModIntro. rred2r.
+         iClear "OBL1 PRM1". clear tid1 γ1 k1.
+        iInv "INV" as "CI" "CI_CLOSE".
+        iEval (unfold client04Inv; red_tl_all; simpl; red_tl) in "CI".
+        iDestruct "CI" as "[%tid1 CI]". iEval (red_tl) in "CI".
+        iDestruct "CI" as "[%tid2' CI]". iEval (red_tl) in "CI".
+        iDestruct "CI" as "[%γ1 CI]". iEval (red_tl) in "CI".
+        iDestruct "CI" as "[%γ2' CI]". iEval (red_tl) in "CI".
+        iDestruct "CI" as "[%k1 CI]". iEval (red_tl) in "CI".
+        iDestruct "CI" as "[%k2' CI]". iEval (red_tl_all; simpl) in "CI".
+        iDestruct "CI" as "(BS1 & BS2 & BM1 & BM2 & [H0 | [_ [H1 | H2]]])".
+        { iDestruct "H0" as "(_ & LIVE & _)". iExFalso; iApply (Lifetime.pending_not_shot with "LIVE"). done. }
+        2:{ iDestruct "H2" as "(PTX & _ & LIVE1 & WS2' & DUTY2' & _)".
+          iExFalso; iApply (AuthExcls.w_w_false with "WS2 WS2'").
+        }
+        iDestruct "H1" as "(PTX & _ & LIVE2 & WS1 & DUTY1 & [(_ & _ & WS2') | WM2])".
+        { iExFalso; iApply (AuthExcls.w_w_false with "WS2 WS2'"). }
+        iPoseProof (AuthExcls.b_w_eq with "BS2 WS2") as "%EQ". clarify.
+        iApply (SCMem_store_fun_spec with "[PTX] [-]"). instantiate (1:=n). auto.
+        { pose proof mask_disjoint_N_Client04_state_tgt; set_solver. }
+        { iFrame. done. }
+        iIntros (rv') "PTX". rred2r. iApply wpsim_tauR. rred2r.
+        iMod (Lifetime.pending_shot with "LIVE2") as "#DEAD2".
+        iMod (duty_fulfill (v:=1+n) with "[DUTY2]") as "DUTY2". iFrame. simpl; red_tl_lifetime; done.
+        iMod (Lifetime.alloc tt) as "[%γ1' LIVE1]".
+        iMod (alloc_obligation 2 2) as "[%obl1 [#OBL1 PC1]]".
+        iPoseProof (pc_split _ _ 1 1 with "[PC1]") as "[PC11 PC12]". done.
+        iMod (pc_drop _ 1 _ _ 1 with "PC11") as "PC11"; auto.
+        iMod (duty_add (v:=1+n) with "[DUTY1 PC11] []") as "DUTY1". iFrame.
+        { instantiate (1 := (dead γ1' tt)%S). iEval (simpl; red_tl_all).
+          iModIntro. iIntros "#D". iModIntro. done.
+        }
+        iPoseProof (duty_tpromise with "[DUTY1]") as "#PRM1". 2: done. simpl; left; auto.
+        iMod (AuthExcls.b_w_update _ _ _ (tid2, obl1, γ1') with "BM2 WM2") as "[BM2 WM2]".
+        iMod (AuthExcls.b_w_update _ _ _ (tid1, obl1, γ1') with "BS1 WS1") as "[BS1 WS1]".
+        clear γ1 k1. rename γ1' into γ1. rename obl1 into k1.
+        iMod ("CI_CLOSE" with "[- WM2]") as "_".
+        { iEval (unfold client04Inv; simpl; red_tl).
+          do 6 (iExists _; red_tl); red_tl_all. 
+          iSplitL "BS1"; [done|]. iSplitL "BS2"; [done|]. iSplitL "BM1"; [done|]. iSplitL "BM2"; [done|].
+          iRight. iSplitR; [done | ]. iRight. simpl. iFrame. iSplitR; [done | ]. iLeft. iFrame.
+        }
+        iApply wpsim_reset. iApply wpsim_base. auto.
+        iApply "CIH". instantiate (1:=(k1, γ1)). iSplitR; iFrame. iModIntro; iFrame.
+        iSplit; [done|]. iSplit; [done|]. iSplit; [done|]. iSplit; [done|]. iSplit; [done | ]. iSplit; done.
+      }
+    }
+    (* Case 2 : x points to 1 *)
+    { iPoseProof (AuthExcls.b_w_eq with "BM2 WM2") as "%EQ". clarify.
+      iDestruct "H1" as "(PTX & #DEADI1 & LIVE2 & WM1 & DUTY1 & [(DUTY2 & PC2 & WS2) | WM2'])"; cycle 1.
+      { iExFalso; iApply (AuthExcls.w_w_false with "WM2 WM2'"). }
+      iMod (pc_drop _ 1 _ _ 3 with "PC2") as "PC2". auto.
+      iPoseProof (pc_split _ _ 1 2 with "PC2") as "[PC21 PC2]".
+      iApply (wpsim_yieldR_gen with "[DUTY2 PC21]"). instantiate (1:=1+n). auto. iFrame.
+      { iApply (pcs_cons_fold). iFrame. }
+      iIntros "DUTY2 CRED".
+      iMod ("CI_CLOSE" with "[- DUTY2 PC2 WS2 LIVEI2]") as "_".
+      { iEval (unfold client04Inv; simpl; red_tl).
+        do 6 (iExists _; red_tl); red_tl_all.
+        iSplitL "BS1"; [done|]. iSplitL "BS2"; [done|]. iSplitL "BM1"; [done|].
+        iSplitL "BM2"; [done|]. iRight. iSplitR; [done | ]. iLeft. simpl.
+        iSplitL "PTX"; [done | ]. iSplitR; [done | ]. iSplitL "LIVE2"; [done | ].
+        iSplitL "WM1"; [done | ]. iSplitL "DUTY1"; [done | ]. iRight. done.
+      }
+      iModIntro. rred2r. clear tid1.
+      iInv "INV" as "CI" "CI_CLOSE".
+      iEval (unfold client04Inv; red_tl_all; simpl; red_tl) in "CI".
+      iDestruct "CI" as "[%tid1 CI]". iEval (red_tl) in "CI".
+      iDestruct "CI" as "[%tid2' CI]". iEval (red_tl) in "CI".
+      iDestruct "CI" as "[%γ1' CI]". iEval (red_tl) in "CI".
+      iDestruct "CI" as "[%γ2' CI]". iEval (red_tl) in "CI".
+      iDestruct "CI" as "[%k1' CI]". iEval (red_tl) in "CI".
+      iDestruct "CI" as "[%k2' CI]". iEval (red_tl_all; simpl) in "CI".
+      iDestruct "CI" as "(BS1 & BS2 & BM1 & BM2 & [H0 | [_ [H1 | H2]]])".
+      { iDestruct "H0" as "(_ & LIVE & _)". iExFalso; iApply (Lifetime.pending_not_shot with "LIVE"). done. }
+      2:{ iDestruct "H2" as "(PTX & _ & _ & WS2' & _)".
+        iExFalso; iApply (AuthExcls.w_w_false with "WS2 WS2'").
+      }
+      iDestruct "H1" as "(PTX & _ & LIVE2 & WS1 & DUTY1 & [(_ & _ & WS2') | WM2])".
+      { iExFalso; iApply (AuthExcls.w_w_false with "WS2 WS2'"). }
+      iPoseProof (AuthExcls.b_w_eq with "BS2 WS2") as "%EQ". clarify.
+      iApply (SCMem_store_fun_spec with "[PTX] [-]"). instantiate (1:=n). auto.
+      { pose proof mask_disjoint_N_Client04_state_tgt; set_solver. }
+      { iFrame. done. }
+      iIntros (rv) "PTX". rred2r. iApply wpsim_tauR. rred2r.
+      iMod (Lifetime.pending_shot with "LIVE2") as "#DEAD2".
+      iMod (Lifetime.pending_shot with "LIVEI2") as "#DEADI2".
+      iMod (duty_fulfill (v:=1+n) with "[DUTY2]") as "DUTY2". iFrame. simpl; red_tl_lifetime; done.
+      clear γ1 k1. iMod (Lifetime.alloc tt) as "[%γ1 LIVE2]".
+      iMod (alloc_obligation 2 2) as "[%k1 [#OBL1 PC1]]".
+      iPoseProof (pc_split _ _ 1 1 with "[PC1]") as "[PC11 PC12]". done.
+      iMod (pc_drop _ 1 _ _ 1 with "PC12") as "PC12"; auto.
+      iMod (duty_add (v:=1+n) with "[DUTY1 PC12] []") as "DUTY1". iFrame.
+      { instantiate (1 := (dead γ1 tt)%S). iEval (simpl; red_tl_all).
+        iModIntro. iIntros "#D". iModIntro. done.
+      }
+      iPoseProof (duty_tpromise with "[DUTY1]") as "#PRM1". 2: done. simpl; left; auto.
+      iMod (AuthExcls.b_w_update _ _ _ (tid2, k1, γ1) with "BM2 WM2") as "[BM2 WM2]".
+      iMod (AuthExcls.b_w_update _ _ _ (tid1, k1, γ1) with "BS1 WS1") as "[BS1 WS1]".
+      iMod ("CI_CLOSE" with "[- WM2]") as "_".
+      { iEval (unfold client04Inv; simpl; red_tl).
+        do 6 (iExists _; red_tl); red_tl_all. 
+        iSplitL "BS1"; [done|]. iSplitL "BS2"; [done|].
+        iSplitL "BM1"; [done|]. iSplitL "BM2"; [done|].
+        iRight. iSplitR; [done | ]. iRight. simpl. iFrame. iSplitR; [done | ]. iLeft. iFrame.
+      }
+      (* Coinduction point *)
+      iClear "DEAD2".
+      iApply wpsim_reset. iStopProof.
+      pose (k1, γ1) as p. replace k1 with (p.1) by ss. replace γ1 with (p.2) by ss. generalize p. clear p.
+      eapply wpsim_coind. auto. clear k1 γ1.
+      ii. destruct a as [k1 γ1].
+      iIntros "[#HG1 #CIH] [(#INV & #MEM & #DEADI & #DEADI1 & #DEADI2 & #OBL1 & #PRM1) WM2]". simpl.
+      iApply (Client04_load_loop_spec2 with "[WM2] [-]").
+      { simpl. red_tl_all; simpl. rewrite red_syn_inv; rewrite red_syn_tgt_interp_as; red_tl_all.
+        iFrame. do 5 (iSplit; [done | ]). done. }
+      iIntros (rv') "(%EQ & %k0 & %γ0 & POST)"; subst. iEval (simpl; red_tl_all; simpl) in "POST".
+      iDestruct "POST" as "(_ & DUTY2 & PC2 & WS2)". rred2r.
+      iPoseProof (pc_split _ _ 1 1 with "PC2") as "[PC21 PC2]".
+      iApply (wpsim_sync_gen with "[DUTY2 PC21]").
+      { instantiate (1:=1+n). auto. }
+      { iFrame. iApply (pcs_cons_fold). iSplitL; done. }
+      iIntros "DUTY2 CRED". iModIntro. lred2r. rred2r. iApply wpsim_tauR. rred2r.
+      iApply wpsim_observe. iIntros (ret). lred2r; rred2r.
+      iApply wpsim_tauL; iApply wpsim_tauR. lred2r; rred2r. iApply wpsim_tauR.
+      do 2 rewrite unfold_iter_eq. lred2r. rred2r.
+      iApply (wpsim_yieldR_gen with "[DUTY2 PC2]"). instantiate (1:=1+n). auto. iFrame.
+      { iApply pcs_cons_fold; iFrame. }
+      iIntros "DUTY2 _". iModIntro. rred2r.
+      iClear "OBL1 PRM1". clear tid1 γ1 γ1' k1.
+      iInv "INV" as "CI" "CI_CLOSE".
+      iEval (unfold client04Inv; red_tl_all; simpl; red_tl) in "CI".
+      iDestruct "CI" as "[%tid1 CI]". iEval (red_tl) in "CI".
+      iDestruct "CI" as "[%tid2' CI]". iEval (red_tl) in "CI".
+      iDestruct "CI" as "[%γ1 CI]". iEval (red_tl) in "CI".
+      iDestruct "CI" as "[%γ2' CI]". iEval (red_tl) in "CI".
+      iDestruct "CI" as "[%k1 CI]". iEval (red_tl) in "CI".
+      iDestruct "CI" as "[%k2' CI]". iEval (red_tl_all; simpl) in "CI".
+      iDestruct "CI" as "(BS1 & BS2 & BM1 & BM2 & [H0 | [_ [H1 | H2]]])".
+      { iDestruct "H0" as "(_ & LIVE & _)". iExFalso; iApply (Lifetime.pending_not_shot with "LIVE"). done. }
+      2:{ iDestruct "H2" as "(PTX & _ & LIVE1 & WS2' & DUTY2' & _)".
+        iExFalso; iApply (AuthExcls.w_w_false with "WS2 WS2'").
+      }
+      iDestruct "H1" as "(PTX & _ & LIVE2 & WS1 & DUTY1 & [(_ & _ & WS2') | WM2])".
+      { iExFalso; iApply (AuthExcls.w_w_false with "WS2 WS2'"). }
+      iPoseProof (AuthExcls.b_w_eq with "BS2 WS2") as "%EQ". clarify.
+      iApply (SCMem_store_fun_spec with "[PTX] [-]"). instantiate (1:=n). auto.
+      { pose proof mask_disjoint_N_Client04_state_tgt; set_solver. }
+      { iFrame. done. }
+      iIntros (rv') "PTX". rred2r. iApply wpsim_tauR. rred2r.
+      iMod (Lifetime.pending_shot with "LIVE2") as "#DEAD2".
+      iMod (duty_fulfill (v:=1+n) with "[DUTY2]") as "DUTY2". iFrame. simpl; red_tl_lifetime; done.
+      iMod (Lifetime.alloc tt) as "[%γ1' LIVE1]".
+      iMod (alloc_obligation 2 2) as "[%obl1 [#OBL1 PC1]]".
+      iPoseProof (pc_split _ _ 1 1 with "[PC1]") as "[PC11 PC12]". done.
+      iMod (pc_drop _ 1 _ _ 1 with "PC11") as "PC11"; auto.
+      iMod (duty_add (v:=1+n) with "[DUTY1 PC11] []") as "DUTY1". iFrame.
+      { instantiate (1 := (dead γ1' tt)%S). iEval (simpl; red_tl_all).
+        iModIntro. iIntros "#D". iModIntro. done.
+      }
+      iPoseProof (duty_tpromise with "[DUTY1]") as "#PRM1". 2: done. simpl; left; auto.
+      iMod (AuthExcls.b_w_update _ _ _ (tid2, obl1, γ1') with "BM2 WM2") as "[BM2 WM2]".
+      iMod (AuthExcls.b_w_update _ _ _ (tid1, obl1, γ1') with "BS1 WS1") as "[BS1 WS1]".
+      clear γ1 k1. rename γ1' into γ1. rename obl1 into k1.
+      iMod ("CI_CLOSE" with "[- WM2]") as "_".
+      { iEval (unfold client04Inv; simpl; red_tl).
+        do 6 (iExists _; red_tl); red_tl_all. 
+        iSplitL "BS1"; [done|]. iSplitL "BS2"; [done|]. iSplitL "BM1"; [done|]. iSplitL "BM2"; [done|].
+        iRight. iSplitR; [done | ]. iRight. simpl. iFrame. iSplitR; [done | ]. iLeft. iFrame.
+      }
+      iApply wpsim_reset. iApply wpsim_base. auto.
+      iApply "CIH". instantiate (1:=(k1, γ1)). iSplitR; iFrame. iModIntro; iFrame.
+      iSplit; [done|]. iSplit; [done|]. iSplit; [done|]. iSplit; [done|]. iSplit; [done | ]. iSplit; done.
+    }
+  Unshelve. all: auto.
+  Qed.
 
   Section INITIAL.
 
@@ -441,77 +1290,41 @@ Section SPEC.
 
     Let idx := 1.
 
-    (* Lemma init_sat E (H_TID : tid1 <> tid2) : *)
-    (*   (OwnM (memory_init_resource Client01.gvs)) *)
-    (*     ∗ *)
-    (*     (WSim.initial_prop *)
-    (*        Client01Spec.module Client01.module *)
-    (*        (Vars:=@sProp STT Γ) (Σ:=Σ) *)
-    (*        (STATESRC:=@SRA.in_subG Γ Σ sub _ _STATESRC) *)
-    (*        (STATETGT:=@SRA.in_subG Γ Σ sub _ _STATETGT) *)
-    (*        (IDENTSRC:=@SRA.in_subG Γ Σ sub _ _IDENTSRC) *)
-    (*        (IDENTTGT:=@SRA.in_subG Γ Σ sub _ _IDENTTGT) *)
-    (*        (ARROWRA:=@_ARROWRA STT Γ Σ TLRAS) *)
-    (*        idx init_ths init_ord) *)
-    (*     ⊢ *)
-    (*     =| 1+idx |=(fairI *)
-    (*                   (IDENTTGT:=@SRA.in_subG Γ Σ sub _ _IDENTTGT) *)
-    (*                   (ARROWRA:=@_ARROWRA STT Γ Σ TLRAS) *)
-    (*                   (1+idx) (ident_tgt:=tgt_ident))={ E, E }=> *)
-    (*         (∃ γk k, *)
-    (*             (inv idx N_Client04 (client01Inv γk k idx)) *)
-    (*               ∗ (tgt_interp_as *)
-    (*                    (STATETGT:=@SRA.in_subG Γ Σ sub _ _STATETGT) *)
-    (*                    (n:=idx) sndl (fun m => (s_memory_black m))) *)
-    (*               ∗ ((own_thread tid1) *)
-    (*                    ∗ (duty *)
-    (*                           (IDENTTGT:=@SRA.in_subG Γ Σ sub _ _IDENTTGT) *)
-    (*                           (ARROWRA:=@_ARROWRA STT Γ Σ TLRAS) *)
-    (*                           (v:=idx) inlp tid1 *)
-    (*                           [(k, 0, ((((dead γk (k : nat)) : @sProp STT Γ idx) ∗ t1_write idx))%S)]) *)
-    (*                    (* ∗ (Duty(tid1) *) *)
-    (*                    (*        (IDENTTGT:=@SRA.in_subG Γ Σ sub _ _IDENTTGT) *) *)
-    (*                    (*        (ARROWRA:=@_ARROWRA STT Γ Σ TLRAS) *) *)
-    (*                    (*        [(k, 0, ((((dead γk (k : nat)) : @sProp STT Γ idx) ∗ t1_write idx))%S)]) *) *)
-    (*                    ∗ ◇[k](2, 1) ∗ (live γk (k : nat) (1/2)) *)
-    (*                 ) *)
-    (*               ∗ *)
-    (*               ((own_thread tid2) ∗ (duty (v:=idx) inlp tid2 [])) *)
-    (*         ). *)
-
     Lemma init_sat E (H_TID : tid1 <> tid2) :
-      (OwnM (memory_init_resource Client01.gvs))
+      (OwnM (memory_init_resource Client04.gvs))
+        ∗ (AuthExcls.rest_gt (0, 0, 0))
         ∗
         (WSim.initial_prop
-           Client01Spec.module Client01.module
+           Client04Spec.module Client04.module
            (Vars:=@sProp STT Γ) (Σ:=Σ)
            (STATESRC:=@SRA.in_subG Γ Σ sub _ _STATESRC)
            (STATETGT:=@SRA.in_subG Γ Σ sub _ _STATETGT)
            (IDENTSRC:=@SRA.in_subG Γ Σ sub _ _IDENTSRC)
            (IDENTTGT:=@SRA.in_subG Γ Σ sub _ _IDENTTGT)
            (ARROWRA:=@_ARROWRA STT Γ Σ TLRAS)
-           idx init_ths init_ord)
+           (1+idx) init_ths init_ord)
         ⊢
-        =| 1+idx |=(⟦syn_fairI (1+idx), 1+idx⟧)={ E, E }=>
-            (∃ γk k,
-                (inv idx N_Client04 (client01Inv γk k idx))
+        =| 2+idx |=(⟦syn_fairI (2+idx), 2+idx⟧)={ E, E }=>
+            (∃ γi γi1 γi2 γs1 γs2 γm1 γm2 k1 k2 γ1 γ2,
+                (inv (1+idx) N_Client04 (client04Inv idx γi γi1 γi2 γs1 γs2 γm1 γm2))
                   ∗ (⟦syn_tgt_interp_as idx sndl (fun m => (s_memory_black m)), 1+idx⟧)
-                  ∗ ((own_thread tid1)
-                       ∗ (⟦Duty(tid1) [(k, 0, ((((dead γk (k : nat)) : @sProp STT Γ idx) ∗ t1_write idx))%S)], idx⟧)
-                       ∗ ◇[k](2, 1) ∗ (live γk (k : nat) (1/2))
-                    )
-                  ∗
-                  ((own_thread tid2) ∗ (⟦Duty(tid2) [], idx⟧))
+                  ∗ ((own_thread tid1) ∗ (live γi1 tt 1) ∗ ○ γm1 (tid1, k2, γ2))
+                  ∗ ((own_thread tid2) ∗ (live γi2 tt 1) ∗ ○ γm2 (tid2, k1, γ1))
             ).
     Proof.
-      iIntros "(MEM & INIT)". rewrite red_syn_fairI.
+      iIntros "(MEM & REST & INIT)". rewrite red_syn_fairI.
       iPoseProof (memory_init_iprop with "MEM") as "[MEM PTS]".
 
-      iMod (alloc_obligation 2 2) as "(%k & #LO & PC)".
-      iMod (Lifetime.alloc k) as "[%γk LIVE]".
-      iPoseProof (Lifetime.pending_split with "[LIVE]") as "[LIVE1 LIVE2]".
-      { iEval (rewrite Qp.div_2). iFrame. }
-      (* iEval (unfold gvs, SCMem.init_gvars; ss) in "PTS". *)
+      iMod (Lifetime.alloc tt) as "[%γi LIVEI]".
+      iMod (Lifetime.alloc tt) as "[%γi1 LIVEI1]".
+      iMod (Lifetime.alloc tt) as "[%γi2 LIVEI2]".
+      (* iAssert (OwnM ((fun k => Auth.frag (Excl.unit : Excl.t (nat * nat * nat))) : AuthExcls.t _))%I as "H".
+      { 
+      } *)
+      iMod (AuthExcls.alloc_gt _ (tid1, 0, 0) with "REST") as "[REST (%γs1 & BS1 & WS1)]".
+      iMod (AuthExcls.alloc_gt _ (tid2, 0, 0) with "REST") as "[REST (%γs2 & BS2 & WS2)]".
+      iMod (AuthExcls.alloc_gt _ (tid1, 0, 0) with "REST") as "[REST (%γm1 & BM1 & WM1)]".
+      iMod (AuthExcls.alloc_gt _ (tid2, 0, 0) with "REST") as "[REST (%γm2 & BM2 & WM2)]".
 
       unfold WSim.initial_prop.
       iDestruct "INIT" as "(INIT0 & INIT1 & INIT2 & INIT3 & INIT4 & INIT5)".
@@ -531,19 +1344,8 @@ Section SPEC.
       iPoseProof (natmap_prop_remove_find _ _ _ H with "INIT3") as "[TH2 INIT3]".
       clear H.
 
-      iEval (replace 2 with (1+1) at 2 by lia) in "PC".
-      iPoseProof (pc_split with "PC") as "[PC1 PC2]".
-      iMod (pc_drop _ 1 _ _ 1 with "PC2") as "PC2". lia.
-      iMod (duty_add (v:=idx) with "[DU1 PC2] []") as "DU1".
-      { iSplitL "DU1". instantiate (1:=[]). iApply "DU1". iFrame. }
-      { instantiate (1:=((dead γk k : sProp idx) ∗ (t1_write idx))%S). simpl. red_tl_all.
-        unfold t1_write. rewrite red_syn_inv. iModIntro. iIntros "#P". auto.
-      }
-      iPoseProof (duty_tpromise with "DU1") as "#PROM1".
-      { ss. eauto. }
-
       iMod (tgt_interp_as_id _ _ (n:=idx) with "[INIT5 MEM]") as "TGT_ST".
-      auto.
+      auto. lia.
       2:{ iExists _. iFrame. instantiate (1:=fun '(_, m) => s_memory_black m). simpl.
           red_tl_all. iFrame.
       }
@@ -556,20 +1358,21 @@ Section SPEC.
       }
       iEval (rewrite Lens.left_unit) in "TGT_ST".
 
-      iMod (FUpd_alloc _ _ _ idx N_Client04 (client01Inv γk k idx) with "[PTS LIVE1]") as "INV1".
+      iMod (FUpd_alloc _ _ _ (1+idx) N_Client04 (client04Inv idx γi γi1 γi2 γs1 γs2 γm1 γm2)
+        with "[PTS LIVEI BS1 WS1 BS2 WS2 BM1 BM2 DU1 DU2]") as "INV1".
       lia.
+      Local Transparent X.
       { simpl. unfold SCMem.init_gvars, gvs. ss. des_ifs. iDestruct "PTS" as "((PT & _) & _)".
-        unfold client01Inv. red_tl_all. rewrite red_syn_until_tpromise.
-        iSplitR. eauto. iSplitR. auto. simpl. iLeft. red_tl_all. iFrame.
-        ss. clarify.
-        (* TODO : make lemmas *)
+        unfold client04Inv. red_tl_all.
+        iExists tid1; red_tl; iExists tid2; red_tl; do 4 (iExists 0; red_tl). simpl; red_tl_all.
+        iSplitL "BS1"; [done | ]. iSplitL "BS2"; [done | ]. iSplitL "BM1"; [done | ]. iSplitL "BM2"; [done | ].
+        iLeft. iFrame.
         Local Transparent SCMem.alloc.
         unfold SCMem.alloc in Heq0. ss. des_ifs.
         Local Opaque SCMem.alloc.
       }
-
-      iModIntro. iExists γk, k. red_tl_all. rewrite red_syn_tgt_interp_as. iFrame.
-      Unshelve. lia.
+      iModIntro. iExists γi, γi1, γi2, γs1, γs2, γm1, γm2. rewrite red_syn_tgt_interp_as. iFrame.
+      iExists 0, 0, 0, 0. iFrame.
     Qed.
 
   End INITIAL.
